Specifications for load-multiple LDM and store-multiple STM have been added to arm_instTheory. Now arm_instTheory provides specifications (with conditional execution and variations of addressing modes) for the following instructions:
  ADC ADD AND B BIC BL CMN CMP EOR LDM LDR MLA MOV MUL MVN ORR RSB
  RSC RSC SBC SMLAL SMULL STM STR SUB SWP TEQ TST UMLAL UMULL

In proving specifications for LDM and STM I found it useful to first
prove the following equivalence:

    |- ARM_RUN P Q =
       !y s.
         P (arm2set' y s) ==>
         ?k. let s' = STATE_ARM_MEM k s in
             Q (arm2set' y s') /\ (arm2set'' y s = arm2set'' y s')

This theorem is called ARM_RUN_SEMANTICS and is part of arm_progTheory.
Above y selects which part of state s is to be translated by the
translation functions arm2set' and arm2set''.


Other changes:

The theorem previously called run_ARM_next___STATE_ARM_MEM is now
called run_arm2set, and the following two theorems have been removed:

val STATE_ARM_MEM_SPLIT = store_thm("STATE_ARM_MEM_SPLIT",
  ``!t1 t2 s. STATE_ARM_MEM (t1 + t2) s =
              STATE_ARM_MEM t1 (STATE_ARM_MEM t2 s)``,
  Induct_on `t1` << [
    SIMP_TAC std_ss [armTheory.STATE_ARM_MEM_def],
    REPEAT GEN_TAC
    \\ `SUC t1 + t2 = SUC (t1 + t2)` by DECIDE_TAC
    \\ ASM_SIMP_TAC std_ss [armTheory.STATE_ARM_MEM_def]]);

val STATE_ARM_MEM_SPLIT___SYM = store_thm("STATE_ARM_MEM_SPLIT___SYM",
  ``!t1 t2 s. STATE_ARM_MEM (t1 + t2) s =
              STATE_ARM_MEM t2 (STATE_ARM_MEM t1 s)``,
  SIMP_TAC arith_ss [GSYM STATE_ARM_MEM_SPLIT]);

The README file has also been updated.

examples/elliptic/sep/arm_instScript.sml
@@ -10,7 +10,8 @@ open HolKernel boolLib bossLib;
 
 open pred_setTheory res_quanTheory wordsTheory arithmeticTheory;
 open arm_rulesTheory arm_rulesLib arm_evalTheory armTheory instructionTheory; 
-open bsubstTheory listTheory rich_listTheory;
+open bsubstTheory listTheory rich_listTheory pairTheory sortingTheory;
+open relationTheory;
 
 open set_sepTheory set_sepLib progTheory arm_progTheory;
 
@@ -640,142 +641,28 @@ val c52TTF = GEN_CONDs (5,2,true,true,false);
 (* Produce theorems to satisfy "cond 2" of IMP_ARM_RUN1                           *)
 (* ----------------------------------------------------------------------------- *)
 
-val arm2set''_THM = prove(
-  ``arm2set'' (rs,ns,st,ud,rt) s =
-    {Reg a (reg a s) |a| ~(a IN rs)} UNION 
-    {Mem a (mem a s) |a| ~(a IN ns)} UNION
-    (if ~ st then {Status (status s)} else {}) UNION
-    (if ~ ud then {Undef s.undefined} else {}) UNION
-    (if ~ rt then {Rest (owrt_visible s)} else {})``,
-  REWRITE_TAC [arm2set''_def,arm2set'_def,EXTENSION,arm2set_def]
-  \\ FULL_SIMP_TAC bool_ss 
-        [IN_UNION,IN_DIFF,IN_INSERT,NOT_IN_EMPTY,GSPECIFICATION,PAIR_EQ]
-  \\ STRIP_TAC \\ EQ_TAC \\ STRIP_TAC << [
-    METIS_TAC [],
-    METIS_TAC [],
-    Cases_on `st` \\ FULL_SIMP_TAC bool_ss [IN_INSERT,NOT_IN_EMPTY],
-    Cases_on `ud` \\ FULL_SIMP_TAC bool_ss [IN_INSERT,NOT_IN_EMPTY],
-    Cases_on `rt` \\ FULL_SIMP_TAC bool_ss [IN_INSERT,NOT_IN_EMPTY],
-    `!k. ?a. x = Reg a (reg a s)` by METIS_TAC []
-    \\ SRW_TAC [] [] \\ METIS_TAC [],    
-    `!k. ?a. x = Mem a (mem a s)` by METIS_TAC []
-    \\ SRW_TAC [] [] \\ METIS_TAC [],
-    Cases_on `st` \\ FULL_SIMP_TAC bool_ss [IN_INSERT,NOT_IN_EMPTY]
-    \\ SRW_TAC [] [],
-    Cases_on `ud` \\ FULL_SIMP_TAC bool_ss [IN_INSERT,NOT_IN_EMPTY]
-    \\ SRW_TAC [] [],    
-    Cases_on `rt` \\ FULL_SIMP_TAC bool_ss [IN_INSERT,NOT_IN_EMPTY]
-    \\ SRW_TAC [] []]);
-
-val arm2set''_EQ = store_thm ("arm2set''_EQ", 
-``!rs ns st ud rt s s'.
-(arm2set'' (rs,ns,st,ud,rt) s = arm2set'' (rs,ns,st,ud,rt) s') = 
-(
-	(!r. (~(r IN rs)) ==> (arm_prog$reg r s = arm_prog$reg r s')) /\
-	(!p. (~(p IN ns)) ==> (arm_prog$mem p s = arm_prog$mem p s')) /\
-	((~st) ==> (status s = status s')) /\
-	((~ud) ==> (s.undefined = s'.undefined)) /\
-	((~rt) ==> (owrt_visible s = owrt_visible s'))
-)``,
-
-SIMP_TAC std_ss [arm2set''_THM, EXTENSION, IN_UNION, IN_DIFF, IN_INSERT, NOT_IN_EMPTY, GSPECIFICATION, prove (``x IN (if c then S1 else S2) =
-												   if c then x IN S1 else x IN S2``, PROVE_TAC[])] THEN
-REPEAT GEN_TAC THEN EQ_TAC THENL [
-	REPEAT STRIP_TAC THEN (
-		CCONTR_TAC THEN
-		Q.PAT_ASSUM `!x. P x` MP_TAC THEN
-		SIMP_TAC std_ss []) THENL [
-
-		Q_TAC EXISTS_TAC `Reg r (arm_prog$reg r s)` THEN
-		FULL_SIMP_TAC std_ss [ARMel_11, ARMel_distinct],
-
-		Q_TAC EXISTS_TAC `Mem p (arm_prog$mem p s)` THEN
-		FULL_SIMP_TAC std_ss [ARMel_11, ARMel_distinct],
-
-		Q_TAC EXISTS_TAC `Status (status s)` THEN
-		FULL_SIMP_TAC std_ss [ARMel_11, ARMel_distinct],
-
-		Q_TAC EXISTS_TAC `Undef s.undefined` THEN
-		FULL_SIMP_TAC std_ss [ARMel_11, ARMel_distinct],
-
-		Q_TAC EXISTS_TAC `Rest (owrt_visible s)` THEN
-		FULL_SIMP_TAC std_ss [ARMel_11, ARMel_distinct]
-	],
-	
-	SIMP_TAC std_ss [] THEN
-	REPEAT STRIP_TAC THEN
-	EQ_TAC THEN REPEAT STRIP_TAC THEN ASM_SIMP_TAC std_ss [ARMel_11, ARMel_distinct]
-])
+val REG_WRITE_r15 = prove(
+  ``!r m n d. ~(15w = n) ==> ((REG_WRITE r m n d) r15 = r r15)``,
+  METIS_TAC [(RW [REG_READ6_def,FETCH_PC_def] o Q.INST [`n2`|->`15w`] o SPEC_ALL) 
+             arm_evalTheory.REG_READ_WRITE_NEQ]);
 
 val REG_READ_WRITE_NEQ2 = prove(
-  ``!n1 n2 r m1 m2 d. ~(n1 = n2) /\ ~(n2 = 15w) ==> 
+  ``!n1 n2 r m1 m2 d. 
+      ~(n1 = n2) ==> 
       (REG_READ (REG_WRITE r m1 n1 d) m2 n2 = REG_READ r m2 n2)``,
-  METIS_TAC [REG_READ6_def,REG_READ_WRITE_NEQ]);
+  REPEAT STRIP_TAC \\ Cases_on `15w = n2`
+  THEN1 ASM_SIMP_TAC std_ss [REG_READ_def,REG_READ_WRITE_NEQ,REG_WRITE_r15]
+  \\ METIS_TAC [REG_READ6_def,REG_READ_WRITE_NEQ]);
 
-val SHAPE_LEMMA_TAC = 
-  EQ_TAC \\ STRIP_TAC \\ ASM_REWRITE_TAC []
-  \\ SRW_TAC [] [reg_def,state_mode_def,set_status_def]
-  \\ CONV_TAC PSR_CONV
-  \\ REWRITE_TAC [GSYM state_mode_def]
-  \\ ASM_SIMP_TAC bool_ss [REG_READ_INC_PC,REG_READ_WRITE_NEQ2];
-
-val SHAPE_LEMMA_TERM_FORMAT =
-  ``(x = Reg a (reg a <|registers := rx; psrs := px; 
-                        memory := v; undefined := v'|>)) /\ bx =
-    (x = Reg a (reg a s)) /\ bx``;
-
-fun MK_SHAPE_LEMMA_TERM (rx,bx) px =
-  subst [``rx:registers``|-> rx,
-         ``px:psrs``    |-> px,
-         ``bx:bool``              |-> bx] SHAPE_LEMMA_TERM_FORMAT;
-
-fun MK_SHAPE_LEMMA (rx,bx) px = prove(MK_SHAPE_LEMMA_TERM (rx,bx) px, SHAPE_LEMMA_TAC);
-
-val n = ``s.psrs``;
-val s = ``set_status (sN,sZ,sC,sV) s``;
-
-val b = (``REG_WRITE s.registers usr 15w z``,``~(a = 15w:word4)``);
-val br = (``REG_WRITE (REG_WRITE s.registers (state_mode s) R1 z') usr 15w z``,``~(a = 15w:word4) /\ ~(a = R1)``);
-val rb = (``REG_WRITE (REG_WRITE s.registers usr 15w z') (state_mode s) R1 z``,``~(a = 15w:word4) /\ ~(a = R1)``);
-
-val i = (``INC_PC s.registers``,``~(a = 15w:word4)``);
-val ir = (``INC_PC (REG_WRITE s.registers (state_mode s) R1 z)``,``~(a = 15w:word4) /\ ~(a = R1)``);
-val ri = (``REG_WRITE (INC_PC s.registers) (state_mode s) R1 z``,``~(a = 15w:word4) /\ ~(a = R1)``);
-val irr = (``INC_PC (REG_WRITE (REG_WRITE s.registers (state_mode s) R1 z') (state_mode s) R2 z)``,``~(a = 15w:word4) /\ ~(a = R1) /\ ~(a = R2)``);
-val rir = (``REG_WRITE (INC_PC (REG_WRITE s.registers (state_mode s) R1 z')) (state_mode s) R2 z``,``~(a = 15w:word4) /\ ~(a = R1) /\ ~(a = R2)``);
-val rri = (``REG_WRITE (REG_WRITE (INC_PC s.registers) (state_mode s) R1 z') (state_mode s) R2 z``,``~(a = 15w:word4) /\ ~(a = R1) /\ ~(a = R2)``);
-
-fun cross f [] ys = []
-  | cross f (x::xs) ys = map (f x) ys @ cross f xs ys;
-
-val SHAPE_REGISTER_LEMMAS = cross MK_SHAPE_LEMMA [b,rb,br,i,ir,ri,irr,rir,rri] [n,s]
-
-val SHAPE_MEM_LEMMA = prove( 
-  ``(x = Mem a (MEM_WRITE_WORD s.memory M2 q a)) /\ 
-    ~(a = M1) /\ ~(a = addr30 M2) =
-    (x = Mem a (mem a s)) /\ ~(a = M1) /\ ~(a = addr30 M2)``,
-  REWRITE_TAC [MEM_WRITE_WORD_def,ADDR30_def,mem_def,GSYM addr30_def]
-  \\ EQ_TAC \\ STRIP_TAC \\ ASM_REWRITE_TAC []    
-  \\ ASM_SIMP_TAC bool_ss [SUBST_def]);
-
-val SHAPE_LEMMAS = map (RW [CONJ_ASSOC]) (SHAPE_MEM_LEMMA::SHAPE_REGISTER_LEMMAS);
-
-val DEFS = [owrt_visible_def,set_status_def,owrt_visible_regs_def,state_mode_def,
-            status_def,statusN_def,statusZ_def,statusC_def,statusV_def,mem_def];
-
-val EXPAND_DEFS_ss = rewrites DEFS
-val CONTRACT_DEFS_ss = rewrites (map GSYM DEFS)
+val SHAPE_ss = rewrites
+  [owrt_visible_def,set_status_def,owrt_visible_regs_def,state_mode_def,
+   status_def,statusN_def,statusZ_def,statusC_def,statusV_def,mem_def,reg_def,
+   REG_READ_WRITE_NEQ2,REG_OWRT_ALL,REG_READ_INC_PC,MEM_WRITE_WORD_def,SUBST_def,
+   ADDR30_def,GSYM addr30_def];
 
 val SHAPE_TAC = 
-  STRIP_TAC
-  \\ REWRITE_TAC [arm2set''_THM]
-  \\ SRW_TAC [] [EXTENSION]
-  \\ SIMP_TAC (bool_ss++EXPAND_DEFS_ss) []
-  \\ SRW_TAC [] []
-  \\ CONV_TAC PSR_CONV
-  \\ SIMP_TAC (bool_ss++CONTRACT_DEFS_ss) [REG_OWRT_ALL]
-  \\ REWRITE_TAC [CONJ_ASSOC]
-  \\ REWRITE_TAC SHAPE_LEMMAS;
+  SIMP_TAC (srw_ss()++SHAPE_ss) [arm2set''_EQ,IN_INSERT,NOT_IN_EMPTY] \\ CONV_TAC PSR_CONV 
+  \\ SIMP_TAC (srw_ss()++SHAPE_ss) [arm2set''_EQ,IN_INSERT,NOT_IN_EMPTY];
 
 val SHAPE_TERM_FORMAT = 
   ``(NEXT_ARM_MEM s = 
@@ -1126,11 +1013,6 @@ val REG_READ_WRITE_NEQ = prove(
 val INC_PC_r15 = prove(
   ``!r. INC_PC r r15 = r r15 + 4w``,
   SRW_TAC [] [INC_PC_def,SUBST_def]);
-
-val REG_WRITE_r15 = prove(
-  ``!r m n d. ~(15w = n) ==> ((REG_WRITE r m n d) r15 = r r15)``,
-  METIS_TAC [(RW [REG_READ6_def,FETCH_PC_def] o Q.INST [`n2`|->`15w`] o SPEC_ALL) 
-             arm_evalTheory.REG_READ_WRITE_NEQ]);
 
 val regs_15w_EQ_reg15 = prove(
   ``!s. s.registers r15 = reg 15w s``,  
@@ -1815,7 +1697,7 @@ val ARM_UNCONDITIONAL_JUMP =
     MATCH_MP th b
   end; 
 
-val _ = save_thm("ARM_B_AL",ARM_UNCONDITIONAL_JUMP);
+val _ = save_thm("arm_B_AL",ARM_UNCONDITIONAL_JUMP);
 
 val ARM_RUN_PUSH_COND = prove(
   ``!P Q g. ARM_RUN (P * cond g) Q ==> ARM_RUN (P * cond g) (Q * cond g)``,
@@ -1843,7 +1725,7 @@ val ARM_CONDITIONAL_JUMP =
     val th = MATCH_MP ARM_RUN_IMP_PROG2 th
   in th end;
 
-val _ = save_thm("ARM_B",ARM_CONDITIONAL_JUMP);
+val _ = save_thm("arm_B",ARM_CONDITIONAL_JUMP);
 
 
 (* procedure calls: ARM_BL *)
@@ -1886,7 +1768,7 @@ val ARM_UNCONDITIONAL_CALL =
     val b = MATCH_MP ARM_RUN_IMP_CALL (RW [lemma] b)
   in b end;
 
-val _ = save_thm("ARM_CALL",ARM_UNCONDITIONAL_CALL);
+val _ = save_thm("arm_BL",ARM_UNCONDITIONAL_CALL);
 
 
 (* procedure returns: MOV_PC *)
@@ -1923,7 +1805,7 @@ val MOV_PC =
     val th = MATCH_MP PROG2_LEMMA (MK_NOP ARM_MOV_NOP)
     val th = MATCH_MP th b 
     val th = RW [GSYM PASS_def] th
-  in save_thm("aMOV_PC",th) end;
+  in save_thm("arm_MOV_PC",th) end;
 
 
 (* ----------------------------------------------------------------------------- *)
@@ -1957,8 +1839,8 @@ val cmps = [(ARM_CMN,ARM_CMN_NOP,"CMN"),
             (ARM_TST,ARM_TST_NOP,"TST"),
             (ARM_TEQ,ARM_TEQ_NOP,"TEQ")];
 
-val _ = store_thms "a" "1" MK_COMPARE1 cmps
-val _ = store_thms "a" "2" MK_COMPARE2 cmps
+val _ = store_thms "arm_" "1" MK_COMPARE1 cmps
+val _ = store_thms "arm_" "2" MK_COMPARE2 cmps
 
 
 (* ----------------------------------------------------------------------------- *)
@@ -1990,8 +1872,8 @@ fun MK_MONOP1 (th,nop) =
 val monops = [(ARM_MOV,ARM_MOV_NOP,"MOV"),
               (ARM_MVN,ARM_MVN_NOP,"MVN")];
 
-val _ = store_thms "a" "1" MK_MONOP1 monops
-val _ = store_thms "a" "2" MK_MONOP2 monops
+val _ = store_thms "arm_" "1" MK_MONOP1 monops
+val _ = store_thms "arm_" "2" MK_MONOP2 monops
 
 
 (* ----------------------------------------------------------------------------- *)
@@ -2072,11 +1954,11 @@ val binops = [(ARM_ADC,ARM_ADC_NOP,"ADC"),
               (ARM_RSC,ARM_RSC_NOP,"SBC"),
               (ARM_SUB,ARM_SUB_NOP,"SUB")];
 
-val _ = store_thms "a" "1" MK_BINOP1 binops
-val _ = store_thms "a" "2" MK_BINOP2 binops
-val _ = store_thms "a" "2'" MK_BINOP2' binops
-val _ = store_thms "a" "2''" MK_BINOP2'' binops
-val _ = store_thms "a" "3" MK_BINOP3 binops
+val _ = store_thms "arm_" "1" MK_BINOP1 binops
+val _ = store_thms "arm_" "2" MK_BINOP2 binops
+val _ = store_thms "arm_" "2'" MK_BINOP2' binops
+val _ = store_thms "arm_" "2''" MK_BINOP2'' binops
+val _ = store_thms "arm_" "3" MK_BINOP3 binops
 
 
 (* ----------------------------------------------------------------------------- *)
@@ -2106,9 +1988,9 @@ val MUL2'' =
     MK_PROG2 (c31TTF,Sris31TTF,[],P31sc') rs (th,ARM_MUL_NOP) BINOP2_INST
   end;
 
-val _ = save_thm("aMUL3",MUL3);
-val _ = save_thm("aMUL2",MUL2);
-val _ = save_thm("aMUL2''",MUL2'');
+val _ = save_thm("arm_MUL3",MUL3);
+val _ = save_thm("arm_MUL2",MUL2);
+val _ = save_thm("arm_MUL2''",MUL2'');
 
 val MLA4 = 
   let
@@ -2145,10 +2027,10 @@ val MLA3'' =
     MK_PROG2 (c41TTF,Sris41TTF,[],P41sc') rs (th,ARM_MLA_NOP) BINOP3_INST
   end;
 
-val _ = save_thm("aMLA4",MLA4);
-val _ = save_thm("aMLA3",MLA3);
-val _ = save_thm("aMLA3'",MLA3');
-val _ = save_thm("aMLA3''",MLA3'');
+val _ = save_thm("arm_MLA4",MLA4);
+val _ = save_thm("arm_MLA3",MLA3);
+val _ = save_thm("arm_MLA3'",MLA3');
+val _ = save_thm("arm_MLA3''",MLA3'');
 
 
 (* ----------------------------------------------------------------------------- *)
@@ -2197,10 +2079,10 @@ val mulls = [(ARM_UMULL,ARM_UMULL_NOP,"UMULL"),
              (ARM_SMULL,ARM_SMULL_NOP,"UMLAL"),
              (ARM_SMULL,ARM_SMULL_NOP,"SMLAL")];
 
-val _ = store_thms "a" "4" MK_MULL4 mulls
-val _ = store_thms "a" "3" MK_MULL3 mulls
-val _ = store_thms "a" "3'" MK_MULL3' mulls
-val _ = store_thms "a" "3''" MK_MULL3'' mulls
+val _ = store_thms "arm_" "4" MK_MULL4 mulls
+val _ = store_thms "arm_" "3" MK_MULL3 mulls
+val _ = store_thms "arm_" "3'" MK_MULL3' mulls
+val _ = store_thms "arm_" "3''" MK_MULL3'' mulls
 
 
 (* ----------------------------------------------------------------------------- *)
@@ -2229,13 +2111,13 @@ val SWP3_NONALIGNED =
     val th = CLEAN_ARM_RULE_C rs th
     val c = ``CONDITION_PASSED2 (sN,sZ,sC,sV) c``
     val th = MK_PROG2 (conds,shape,insts,prog) rs (th,nop) i
-  in save_thm("aSWP3_NONALIGNED",th) end;
+  in save_thm("arm_SWP3_NONALIGNED",th) end;
 
 val SWP3 = 
   let
     val th = Q.INST [`z`|->`addr32 z`] SWP3_NONALIGNED
     val th = RW [ADDRESS_ROTATE,addr30_addr32,GSYM R30_def] th    
-  in save_thm("aSWP3",th) end;
+  in save_thm("arm_SWP3",th) end;
 
 val SWP2_NONALIGNED = 
   let
@@ -2247,13 +2129,13 @@ val SWP2_NONALIGNED =
     val insts = [``M2:word32``|->``x2:word32``]
     val i = SWP2_INST
     val th = MK_PROG2 (conds,shape,insts,prog) rs (th,nop) i
-  in save_thm("aSWP2_NONALIGNED",th) end;
+  in save_thm("arm_SWP2_NONALIGNED",th) end;
 
 val SWP2 = 
   let
     val th = Q.INST [`y`|->`addr32 y`] SWP2_NONALIGNED
     val th = RW [ADDRESS_ROTATE,addr30_addr32,GSYM R30_def] th    
-  in save_thm("aSWP2",th) end;
+  in save_thm("arm_SWP2",th) end;
 
 
 (* ----------------------------------------------------------------------------- *)
@@ -2305,9 +2187,9 @@ val STR_NONALIGNED =
     val th = MOVE_STAR_RULE `a*b*s*c*y` `a*b*y*s*c` th
     val imp = MATCH_MP PROG2_LEMMA (MK_NOP nop)
     val th = MATCH_MP imp th 
-  in save_thm("aSTR_NONALIGNED",th) end;
+  in save_thm("arm_STR_NONALIGNED",th) end;
 
-val STR = save_thm("aSTR",AM2_ALIGN_ADDRESSES `y` STR_NONALIGNED);
+val STR = save_thm("arm_STR",AM2_ALIGN_ADDRESSES `y` STR_NONALIGNED);
 
 val LDR_NONALIGNED =
   let
@@ -2317,9 +2199,9 @@ val LDR_NONALIGNED =
     val insts = [``M2:word32``|->``(ADDR_MODE2_ADDR' a_mode x1):word32``]
     val i = STR_INST
     val th = MK_PROG2 (conds,shape,insts,prog) rs (th,nop) i
-  in save_thm("aLDR_NONALIGNED",th) end;
+  in save_thm("arm_LDR_NONALIGNED",th) end;
 
-val LDR = save_thm("aLDR",AM2_ALIGN_ADDRESSES `y` LDR_NONALIGNED);
+val LDR = save_thm("arm_LDR",AM2_ALIGN_ADDRESSES `y` LDR_NONALIGNED);
 
 val LDR1_NONALIGNED =
   let
@@ -2342,9 +2224,9 @@ val LDR1_NONALIGNED =
     val th = MOVE_STAR_RULE `b*y*s*p*c` `b*y*c*s*p` th
     val th' = MATCH_MP PROG2_LEMMA (MK_NOP nop)
     val th = MATCH_MP th' th
-  in save_thm("aLDR1_NONALIGNED",th) end;
+  in save_thm("arm_LDR1_NONALIGNED",th) end;
 
-val LDR1 = save_thm("aLDR1",AM2_ALIGN_ADDRESSES `y` LDR1_NONALIGNED);
+val LDR1 = save_thm("arm_LDR1",AM2_ALIGN_ADDRESSES `y` LDR1_NONALIGNED);
 
 val LDR_PC_LEMMA = prove(
   ``!regs m x. REG_WRITE (INC_PC regs) m 15w x = REG_WRITE regs usr 15w x``,
@@ -2379,454 +2261,1568 @@ val LDR_PC =
     val imp = MATCH_MP PROG2_LEMMA (MK_NOP nop)
     val imp = AM2_ALIGN_ADDRESSES `x:word32` imp   
     val th = MATCH_MP imp th
-  in save_thm("aLDR_PC",th) end;
+  in save_thm("arm_LDR_PC",th) end;
+
+
+(* ----------------------------------------------------------------------------- *)
+(* General tools                                                                 *)
+(* ----------------------------------------------------------------------------- *)
+
+val ARM_PROG2_EQ = let
+  val th = Q.SPECL [`P`,`[cmd]`,`Q`,`Q'`,`f`] ARM_PROG_INTRO
+  val th = SIMP_RULE (std_ss++sep_ss) [LENGTH,ms_def,pcINC_def,wLENGTH_def] th
+  val th = SIMP_RULE std_ss [ARM_RUN_SEMANTICS,ARMpc_def,STAR_ASSOC,R30_def,SEP_DISJ_def,LET_DEF] th
+  in GSYM th end;
+
+val ARM_PROG1_EQ = let
+  val th = Q.INST [`Q'`|->`SEP_F`] ARM_PROG2_EQ
+  val th = SIMP_RULE (bool_ss++sep_ss) [ARM_PROG_FALSE_POST,SEP_F_def,LET_DEF] th
+  in th end;
+
+val STATE_ARM_MEM_1 = 
+  REWRITE_CONV [GSYM (EVAL ``SUC 0``),STATE_ARM_MEM_def]``STATE_ARM_MEM 1 s``;
+
+val ARM_PROG_INIT_TAC = 
+  REWRITE_TAC [ARM_PROG1_EQ,ARM_PROG2_EQ,PASS_def] \\ REPEAT STRIP_TAC
+  \\ Q.EXISTS_TAC `1` \\ REWRITE_TAC [STATE_ARM_MEM_1];
+
+
+(* ----------------------------------------------------------------------------- *)
+(* Semantics of ``R a1 x1  * ... * R an xn * ms b1 y1 * ... * ms bm ym * ...``   *)
+(* ----------------------------------------------------------------------------- *)
+
+val xR_list_def = Define `
+  (xR_list [] = emp) /\
+  (xR_list ((r,NONE)::xs) = ~R r * xR_list xs) /\
+  (xR_list ((r,SOME x)::xs) = R r x * xR_list xs)`;
+
+val xR_list_sem_def = Define `
+  (xR_list_sem [] s = T) /\
+  (xR_list_sem ((r,NONE)::xs) s = xR_list_sem xs s) /\
+  (xR_list_sem ((r,SOME x)::xs) s = (reg r s = x) /\ xR_list_sem xs s)`;
+
+val xR_list_lemma = prove(
+  ``((R r x * P) (arm2set' (rs,ns,st,ud,rt) s) = 
+     (reg r s = x) /\ r IN rs /\ P (arm2set' (rs DELETE r,ns,st,ud,rt) s)) /\ 
+    ((~R r * P) (arm2set' (rs,ns,st,ud,rt) s) = 
+     r IN rs /\ P (arm2set' (rs DELETE r,ns,st,ud,rt) s))``,
+  SIMP_TAC (std_ss++sep2_ss) [R_def,SEP_HIDE_THM] 
+  \\ SIMP_TAC std_ss [SEP_EXISTS,one_STAR,IN_arm2set']
+  \\ METIS_TAC [DELETE_arm2set']);
+
+val xR_list_thm = prove(
+  ``!xs P rs ns st ud rt. 
+      (xR_list xs * P) (arm2set' (rs,ns,st,ud,rt) s) = 
+      xR_list_sem xs s /\ ALL_DISTINCT (MAP FST xs) /\ 
+      P (arm2set' (rs DIFF (LIST_TO_SET (MAP FST xs)),ns,st,ud,rt) s) /\
+      (LIST_TO_SET (MAP FST xs)) SUBSET rs``,
+  Induct
+  THEN1 SRW_TAC [sep_ss] [xR_list_def,xR_list_sem_def,MAP,ALL_DISTINCT]
+  \\ REPEAT STRIP_TAC \\ Cases_on `h` \\ Cases_on `r`
+  \\ SIMP_TAC bool_ss [MAP,ALL_DISTINCT,pairTheory.FST,xR_list_sem_def,xR_list_def]
+  \\ ASM_REWRITE_TAC [GSYM STAR_ASSOC,xR_list_lemma]
+  \\ `LIST_TO_SET (q::MAP FST xs) SUBSET rs =
+      q IN rs /\ LIST_TO_SET (MAP FST xs) SUBSET rs` by SRW_TAC [] []
+  \\ `rs DIFF LIST_TO_SET (q::MAP FST xs) =
+      rs DELETE q DIFF LIST_TO_SET (MAP FST xs)` by 
+         SRW_TAC [] [EXTENSION,IN_DIFF,IN_DELETE,CONJ_ASSOC]
+  \\ `LIST_TO_SET (MAP FST xs) SUBSET rs DELETE q =
+      ~MEM q (MAP FST xs) /\ LIST_TO_SET (MAP FST xs) SUBSET rs` by 
+         (SRW_TAC [] [SUBSET_DEF,IN_DELETE] \\ METIS_TAC [])
+  \\ ASM_REWRITE_TAC [] \\ METIS_TAC []);
+
+val _ = Hol_datatype `
+  xM_option = xM_seq of word32 list | xM_blank of num`;
+
+val xM_list_def = Define `
+  (xM_list [] = emp) /\
+  (xM_list ((a,xM_blank n)::xs) = blank_ms a n * xM_list xs) /\
+  (xM_list ((a,xM_seq x)::xs) = ms a x * xM_list xs)`;
+
+val ms_sem_def = Define `
+  (ms_sem a [] s = T) /\ 
+  (ms_sem a (x::xs) s = (mem a s = x) /\ ms_sem (a+1w) xs s)`;
+
+val xM_list_sem_def = Define `
+  (xM_list_sem [] s = T) /\
+  (xM_list_sem ((a,xM_blank n)::xs) s = n <= 2**30 /\ xM_list_sem xs s) /\
+  (xM_list_sem ((a,xM_seq x)::xs) s = 
+     ms_sem a x s /\ LENGTH x <= 2**30 /\ xM_list_sem xs s)`;
+
+val ms_address_set_def = Define `
+  (ms_address_set a 0 = ({}:word30 set)) /\ 
+  (ms_address_set a (SUC n) = a INSERT ms_address_set (a+1w) n)`;
+
+val xM_list_addresses_def = Define `
+  (xM_list_addresses [] = []) /\
+  (xM_list_addresses ((a,xM_blank n)::xs) = 
+    ms_address_set a n :: xM_list_addresses xs) /\
+  (xM_list_addresses ((a,xM_seq x)::xs) = 
+    ms_address_set a (LENGTH x) :: xM_list_addresses xs)`;
+
+val xM_list_address_set_def = Define `
+  xM_list_address_set xs = FOLDR $UNION EMPTY (xM_list_addresses xs)`;
+
+val ALL_DISJOINT_def = Define `
+  (ALL_DISJOINT [] = T) /\
+  (ALL_DISJOINT (x::xs) = EVERY (\y. DISJOINT x y) xs /\ ALL_DISJOINT xs)`;
+
+val IN_ms_address_set_ADD1 = prove(
+  ``!xs a b. a IN (ms_address_set b xs) = (a+1w) IN (ms_address_set (b+1w) xs)``,
+  Induct \\ SIMP_TAC std_ss [ms_address_set_def,NOT_IN_EMPTY,IN_INSERT,WORD_EQ_ADD_RCANCEL]
+  \\ METIS_TAC []);
+
+val ms_address_set_no_overlap_lemma = prove(
+  ``!k n. k <= n /\ n < 2**30 ==> ~((a + n2w n) IN (ms_address_set a k))``,
+  Induct \\ FULL_SIMP_TAC std_ss [ms_address_set_def,NOT_IN_EMPTY,IN_INSERT]
+  \\ REPEAT STRIP_TAC 
+  THEN1 (FULL_SIMP_TAC (std_ss++wordsLib.SIZES_ss) [WORD_ADD_RID_UNIQ,n2w_11]
+         \\ `~(0 = n)` by DECIDE_TAC \\ METIS_TAC [LESS_MOD])
+  \\ `k <= n - 1 /\ n - 1 < 1073741824` by DECIDE_TAC
+  \\ `~((a + n2w (n-1)) IN (ms_address_set a k))` by METIS_TAC []
+  \\ `!k a b. (b + 1w) IN (ms_address_set (a + 1w) k) = b IN (ms_address_set a k)` by
+         (Induct \\ SRW_TAC [] [ms_address_set_def,WORD_EQ_ADD_RCANCEL])
+  \\ `n = (n-1)+1` by DECIDE_TAC 
+  \\ `a + n2w ((n-1)+1) IN ms_address_set (a + 1w) k` by METIS_TAC []
+  \\ FULL_SIMP_TAC std_ss [GSYM word_add_n2w,WORD_ADD_ASSOC]
+  \\ METIS_TAC []);
+
+val ms_address_set_no_overlap = prove(
+  ``!k h a. SUC k <= 2**30 ==> ~(a IN (ms_address_set (a+1w:word30) k))``,
+  SIMP_TAC bool_ss [LENGTH,GSYM LESS_EQ] \\ REPEAT STRIP_TAC
+  \\ `k <= 2 ** 30 - 1 /\ 2 ** 30 - 1 < 2 ** 30` by DECIDE_TAC
+  \\ `~((a + n2w (2 ** 30 - 1) + 1w) IN (ms_address_set (a + 1w) k))` 
+           by METIS_TAC [ms_address_set_no_overlap_lemma,IN_ms_address_set_ADD1] 
+  \\ `2 ** 30 - 1 + 1 = 2 ** 30` by DECIDE_TAC
+  \\ `n2w (2 ** 30) = 0w:word30` by SIMP_TAC (std_ss++wordsLib.SIZES_ss) [n2w_11]
+  \\ FULL_SIMP_TAC bool_ss [GSYM WORD_ADD_ASSOC,word_add_n2w,WORD_ADD_0]);
+
+val IN_ms_address_set = prove(
+  ``!n a b. b IN ms_address_set a n = ?k. k < n /\ (b = n2w k + a)``,
+  Induct \\ REWRITE_TAC [ms_address_set_def,NOT_IN_EMPTY,DECIDE ``~(k<0)``,IN_INSERT]
+  \\ REPEAT STRIP_TAC \\ EQ_TAC \\ REPEAT STRIP_TAC \\ ASM_REWRITE_TAC []
+  THEN1 (Q.EXISTS_TAC `0` \\ ASM_REWRITE_TAC [WORD_ADD_0] \\ DECIDE_TAC) << [
+    Q.PAT_ASSUM `!a:'a. b:bool` IMP_RES_TAC
+    \\ `SUC k < SUC n` by DECIDE_TAC \\ Q.EXISTS_TAC `SUC k`
+    \\ ASM_REWRITE_TAC [ADD1,GSYM word_add_n2w] \\ METIS_TAC [WORD_ADD_ASSOC,WORD_ADD_COMM],
+    Cases_on `k` \\ REWRITE_TAC [WORD_ADD_0] 
+    \\ DISJ2_TAC \\ Q.EXISTS_TAC `n'` \\ `n' < n` by DECIDE_TAC 
+    \\ ASM_REWRITE_TAC [ADD1,GSYM word_add_n2w] \\ METIS_TAC [WORD_ADD_ASSOC,WORD_ADD_COMM]]);
+      
+val xM_list_lemma_LEMMA1 = prove(
+  ``!a n ns. ms_address_set (a + 1w) n SUBSET ns DELETE a ==> SUC n <= 2 ** 30``,
+  REWRITE_TAC [SUBSET_DEF,IN_DELETE] \\ REPEAT STRIP_TAC \\ CCONTR_TAC
+  \\ `2 ** 30 <= n` by DECIDE_TAC  
+  \\ `a IN ms_address_set (a + 1w) n` by ALL_TAC << [    
+    REWRITE_TAC [IN_ms_address_set] \\ Q.EXISTS_TAC `2**30-1`
+    \\ `1 <= 2**30` by EVAL_TAC
+    \\ ASM_SIMP_TAC bool_ss [LESS_EQ,ADD1,SUB_ADD,WORD_ADD_ASSOC]
+    \\ `!b. b + a + 1w = b + 1w + a` by METIS_TAC [WORD_ADD_COMM,WORD_ADD_ASSOC]
+    \\ ASM_SIMP_TAC bool_ss [word_add_n2w,SUB_ADD]
+    \\ ONCE_REWRITE_TAC [GSYM n2w_mod]
+    \\ ASM_SIMP_TAC (std_ss++wordsLib.SIZES_ss) [WORD_ADD_0],
+    METIS_TAC []]);
+
+val xM_list_lemma_LEMMA2 = prove(
+  ``!a n ns. SUC n <= 2 ** 30 ==> ~(a IN ms_address_set (a + 1w) n)``,
+  SIMP_TAC bool_ss [IN_ms_address_set] \\ REPEAT STRIP_TAC
+  \\ Cases_on `k < n` \\ ASM_REWRITE_TAC [WORD_ADD_ASSOC]
+  \\ `!b. b + a + 1w = a + (b + 1w)` by METIS_TAC [WORD_ADD_COMM,WORD_ADD_ASSOC]
+  \\ ASM_REWRITE_TAC [word_add_n2w] \\ ONCE_REWRITE_TAC [EQ_SYM_EQ]
+  \\ `k + 1 < 2**30` by DECIDE_TAC
+  \\ FULL_SIMP_TAC (std_ss++wordsLib.SIZES_ss) [WORD_ADD_RID_UNIQ,n2w_11]);
+
+val xM_list_lemma1 = prove(
+  ``!xs a rs ns st ud rt P.
+      ((ms a xs * P) (arm2set' (rs,ns,st,ud,rt) s) = 
+       (ms_sem a xs s) /\ LENGTH xs <= 2**30 /\
+       ms_address_set a (LENGTH xs) SUBSET ns /\ 
+       P (arm2set' (rs,ns DIFF ms_address_set a (LENGTH xs),st,ud,rt) s))``,
+  Induct THEN1 SRW_TAC [sep_ss] [ms_def,ms_sem_def,ms_address_set_def]
+  \\ REWRITE_TAC [ms_def,ms_sem_def,GSYM STAR_ASSOC,M_def,one_STAR]
+  \\ REPEAT STRIP_TAC \\ ASM_REWRITE_TAC [IN_arm2set']
+  \\ Cases_on `~(h = mem a s)` THEN1 METIS_TAC []
+  \\ FULL_SIMP_TAC bool_ss [LENGTH]
+  \\ ASM_SIMP_TAC bool_ss [DELETE_arm2set',ms_address_set_def,LENGTH]
+  \\ `!k. ns DELETE a DIFF ms_address_set (a + 1w) k =
+          ns DIFF (a INSERT ms_address_set (a + 1w) k)` by 
+        SRW_TAC [] [EXTENSION,IN_DELETE,IN_DIFF,CONJ_ASSOC]
+  \\ EQ_TAC \\ ASM_SIMP_TAC bool_ss [] \\ STRIP_TAC
+  \\ IMP_RES_TAC xM_list_lemma_LEMMA1 \\ ASM_REWRITE_TAC []
+  \\ FULL_SIMP_TAC bool_ss [IN_INSERT,SUBSET_DEF,IN_DELETE] THEN1 METIS_TAC []  
+  \\ STRIP_TAC THEN1 DECIDE_TAC
+  \\ IMP_RES_TAC xM_list_lemma_LEMMA2 \\ ASM_REWRITE_TAC []);
+
+val xM_list_lemma2 = prove(
+  ``!n a rs ns st ud rt P.
+      ((blank_ms a n * P) (arm2set' (rs,ns,st,ud,rt) s) = 
+       n <= 2**30 /\ ms_address_set a n SUBSET ns /\ 
+       P (arm2set' (rs,ns DIFF ms_address_set a n,st,ud,rt) s))``,
+  Induct THEN1 SRW_TAC [sep_ss] [blank_ms_def,ms_address_set_def]
+  \\ REWRITE_TAC [blank_ms_def,GSYM STAR_ASSOC,M_def,one_STAR]
+  \\ SIMP_TAC (bool_ss++sep2_ss) [SEP_HIDE_THM] 
+  \\ SIMP_TAC bool_ss [SEP_EXISTS_THM,M_def,one_STAR,GSYM STAR_ASSOC]
+  \\ REPEAT STRIP_TAC \\ ASM_REWRITE_TAC [IN_arm2set']
+  \\ FULL_SIMP_TAC bool_ss []
+  \\ ASM_SIMP_TAC bool_ss [DELETE_arm2set',ms_address_set_def]
+  \\ `!k. ns DELETE a DIFF ms_address_set (a + 1w) k =
+          ns DIFF (a INSERT ms_address_set (a + 1w) k)` by 
+        SRW_TAC [] [EXTENSION,IN_DELETE,IN_DIFF,CONJ_ASSOC]
+  \\ EQ_TAC \\ ASM_SIMP_TAC bool_ss [] \\ STRIP_TAC
+  \\ IMP_RES_TAC xM_list_lemma_LEMMA1 \\ ASM_REWRITE_TAC []
+  \\ FULL_SIMP_TAC bool_ss [IN_INSERT,SUBSET_DEF,IN_DELETE] THEN1 METIS_TAC []  
+  \\ STRIP_TAC THEN1 DECIDE_TAC
+  \\ IMP_RES_TAC xM_list_lemma_LEMMA2 \\ ASM_REWRITE_TAC []);
+
+val EVERY_DISJOINT = prove(
+  ``!xs x. EVERY (\y. DISJOINT x y) xs = DISJOINT x (FOLDR $UNION {} xs)``,
+  Induct \\ ASM_SIMP_TAC std_ss [EVERY_DEF,FOLDR,DISJOINT_EMPTY]
+  \\ SRW_TAC [] [DISJOINT_DEF,EXTENSION] \\ METIS_TAC []);
+
+val xM_list_thm = prove(
+  ``!xs P rs ns st ud rt.
+      ((xM_list xs * P) (arm2set' (rs,ns,st,ud,rt) s) = 
+       xM_list_sem xs s /\ ALL_DISJOINT (xM_list_addresses xs) /\ 
+       P (arm2set' (rs,ns DIFF (xM_list_address_set xs),st,ud,rt) s) /\
+       xM_list_address_set xs SUBSET ns)``,
+  Induct
+  THEN1 SRW_TAC [sep_ss] [xM_list_def,xM_list_sem_def,MAP,ALL_DISJOINT_def,
+                          xM_list_address_set_def,xM_list_addresses_def]
+  \\ REPEAT STRIP_TAC \\ Cases_on `h` \\ Cases_on `r`
+  \\ SIMP_TAC bool_ss [MAP,ALL_DISJOINT_def,pairTheory.FST,xM_list_sem_def,xM_list_def,
+                       xM_list_addresses_def,xM_list_address_set_def,FOLDR]
+  \\ FULL_SIMP_TAC bool_ss [GSYM xM_list_address_set_def]
+  \\ ASM_SIMP_TAC std_ss [xM_list_lemma1,xM_list_lemma2,GSYM STAR_ASSOC]
+  \\ SIMP_TAC bool_ss [EVERY_DISJOINT,GSYM xM_list_address_set_def] 
+  \\ REWRITE_TAC [prove(``!x:'a set y z. x DIFF y DIFF z = x DIFF (y UNION z)``, 
+                  SRW_TAC [] [EXTENSION,IN_UNION,IN_DIFF,CONJ_ASSOC])]
+  \\ `!x y z:word30 set. 
+      DISJOINT x y /\ x UNION y SUBSET z = y SUBSET z DIFF x /\ x SUBSET z` by
+        (SRW_TAC [] [SUBSET_DEF,DISJOINT_DEF,EXTENSION] \\ METIS_TAC [])
+  \\ EQ_TAC \\ ASM_SIMP_TAC std_ss [] \\ METIS_TAC []);
+
+val rest_list_def = Define `
+  rest_list (st,ud,rt,cd) (x,y,z,b) = 
+    (if st then S x else emp) * 
+    (if ud then one (Undef y) else emp) * 
+    (if rt then one (Rest z) else emp) * 
+    (if cd then cond b else emp)`;
+
+val rest_list_sem_def = Define `
+  rest_list_sem (st,ud,rt,cd) (x,y,z,b) s = 
+    (if st then (status s = x) else T) /\ 
+    (if ud then (s.undefined = y) else T) /\
+    (if rt then (owrt_visible s = z) else T) /\ 
+    (if cd then b else T)`;
+
+val rest_list_thm = prove(
+  ``!st ud rt cd x y z b P rs ns st' ud' rt'. 
+      (rest_list (st,ud,rt,cd) (x,y,z,b) * P) (arm2set' (rs,ns,st',ud',rt') s) = 
+      rest_list_sem (st,ud,rt,cd) (x,y,z,b) s /\ 
+      (st ==> st') /\ (ud ==> ud') /\ (rt ==> rt') /\
+      P (arm2set' (rs,ns,~st /\ st',~ud /\ ud',~rt /\ rt') s)``,
+  REPEAT STRIP_TAC
+  \\ REWRITE_TAC [rest_list_def,rest_list_sem_def,
+       prove(``!cd b. (if cd then cond b else emp) = cond (cd ==> b)``,SRW_TAC [sep_ss][])] 
+  \\ Cases_on `st` \\ SIMP_TAC (bool_ss++sep_ss) [] \\ Cases_on `x = status s` 
+  \\ Cases_on `ud` \\ SIMP_TAC (bool_ss++sep_ss) [] \\ Cases_on `y = s.undefined` 
+  \\ Cases_on `rt` \\ SIMP_TAC (bool_ss++sep_ss) [] \\ Cases_on `z = owrt_visible s` 
+  \\ ASM_SIMP_TAC bool_ss [GSYM STAR_ASSOC,S_def,one_STAR,IN_arm2set',DELETE_arm2set',cond_STAR]
+  \\ EQ_TAC \\ ASM_SIMP_TAC bool_ss []);
+
+val emp_list_thm = prove(
+  ``!s rs ns st ud rt.
+       emp (arm2set' (rs,ns,st,ud,rt) s) = (rs = {}) /\ (ns = {}) /\ ~st /\ ~ud /\ ~rt``,
+  SIMP_TAC std_ss [emp_def,arm2set'_def]
+  \\ REPEAT STRIP_TAC
+  \\ Cases_on `st` THEN1 SRW_TAC [] [EXTENSION]
+  \\ Cases_on `ud` THEN1 SRW_TAC [] [EXTENSION]
+  \\ Cases_on `rt` THEN1 SRW_TAC [] [EXTENSION]
+  \\ SRW_TAC [] [EXTENSION,GSPECIFICATION]);
+
+val rest_emp_list_thm = prove(
+  ``!st ud rt xs x y z b P rs ns st' ud' rt'. 
+      (rest_list (st,ud,rt,cd) (x,y,z,b)) (arm2set' (rs,ns,st',ud',rt') s) = 
+      rest_list_sem (st,ud,rt,cd) (x,y,z,b) s /\ 
+      (rs = {}) /\ (ns = {}) /\ (st = st') /\ (ud = ud') /\ (rt = rt')``,
+  REPEAT STRIP_TAC  
+  \\ CONV_TAC ((RATOR_CONV o RAND_CONV o RATOR_CONV) 
+               (ONCE_REWRITE_CONV [(GSYM o CONJUNCT2 o SPEC_ALL) emp_STAR]))
+  \\ REWRITE_TAC [rest_list_thm,emp_list_thm]
+  \\ Cases_on `st` \\ Cases_on `st'` \\ Cases_on `ud` \\ Cases_on `ud'`
+  \\ Cases_on `rt` \\ Cases_on `rt'` \\ SIMP_TAC bool_ss []);
+
+val spec_list_def = Define `
+  spec_list xs ys (st,x) (ud,y) (rt,z) (cd,b) = 
+    xR_list xs * xM_list ys * rest_list (st,ud,rt,cd) (x,y,z,b)`;
+
+val spec_list_select_def = Define `
+  spec_list_select (xs,ys,st,ud,rt) =
+    (LIST_TO_SET (MAP FST xs),xM_list_address_set ys,st,ud,rt)`;
+  
+val spec_list_sem_def = Define `
+  spec_list_sem xs ys (st,x) (ud,y) (rt,z) (cd,b) q s =
+    xR_list_sem xs s /\ xM_list_sem ys s /\ rest_list_sem (st,ud,rt,cd) (x,y,z,b) s /\ 
+    ALL_DISTINCT (MAP FST xs) /\ ALL_DISJOINT (xM_list_addresses ys) /\
+    (q = spec_list_select (xs,ys,st,ud,rt))`;
+  
+val spec_list_thm = prove(
+  ``!xs ys st ud rt cd q s.
+      (spec_list xs ys st ud rt cd) (arm2set' q s) = 
+      spec_list_sem xs ys st ud rt cd q s``,
+  REPEAT STRIP_TAC
+  \\ `?rs ns st' ud' rt'. q = (rs,ns,st',ud',rt')` by METIS_TAC [pairTheory.PAIR]
+  \\ `?st' x. st = (st',x)` by METIS_TAC [pairTheory.PAIR]
+  \\ `?ud' y. ud = (ud',y)` by METIS_TAC [pairTheory.PAIR]
+  \\ `?rt' z. rt = (rt',z)` by METIS_TAC [pairTheory.PAIR]
+  \\ `?cd' b. cd = (cd',b)` by METIS_TAC [pairTheory.PAIR]
+  \\ ASM_SIMP_TAC bool_ss [spec_list_def,GSYM STAR_ASSOC,xR_list_thm,xM_list_thm]
+  \\ ASM_SIMP_TAC bool_ss [rest_emp_list_thm,
+       prove(``(x DIFF y = {}) = x SUBSET y``,
+       SRW_TAC [] [EXTENSION,SUBSET_DEF] \\ METIS_TAC [])]
+  \\ REWRITE_TAC [spec_list_sem_def,pairTheory.PAIR_EQ,spec_list_select_def]
+  \\ REWRITE_TAC [SET_EQ_SUBSET,GSYM CONJ_ASSOC]
+  \\ EQ_TAC \\ SIMP_TAC std_ss []);
+
+(* function for instantiation *)
+
+val LIST_TO_SET_CLAUSES = prove(
+  ``!x xs. (LIST_TO_SET [] = {}) /\ (LIST_TO_SET (x::xs) = x INSERT LIST_TO_SET xs)``,
+  SRW_TAC [] [EXTENSION]);
+
+val UNION_APPEND = prove(
+  ``!x y z. (x INSERT y) UNION z = x INSERT (y UNION z)``,
+  SRW_TAC [] [EXTENSION,DISJ_ASSOC]);
+
+val spec_list_expand_ss = rewrites 
+  [spec_list_def,xR_list_def,xM_list_def,rest_list_def,spec_list_sem_def,
+   xR_list_sem_def,xM_list_sem_def,rest_list_sem_def,ms_sem_def,
+   xM_list_addresses_def,ms_address_set_def,LIST_TO_SET_CLAUSES,spec_list_select_def,
+   xM_list_address_set_def,FOLDR,UNION_EMPTY,UNION_APPEND,GSYM CONJ_ASSOC,ms_def,
+   MAP,FST,STAR_ASSOC,EVAL ``SUC 0 <= 2**30``,LENGTH];
+
+fun sep_pred_semantics (xs,ys,st,ud,rt,cd) = let
+  val th = Q.SPECL [xs,ys,st,ud,rt,cd] spec_list_thm
+  val th = SIMP_RULE (bool_ss++sep_ss++spec_list_expand_ss) [] th
+  in th end;
+
+(* example *)
+
+val xs = `[(a1,SOME x1);(a2,SOME x2);(a3,SOME x3);(a4,NONE);(a5,NONE);(a6,NONE)]`;
+val ys = `[(b1,xM_seq [y1]);(b2,xM_seq [y2]);(b3,xM_seq y3);(b4,xM_blank k4)]`;
+val st = `(T,st)`;
+val ud = `(T,ud)`;
+val rt = `(F,rt)`;
+val cd = `(T,g)`;
+val th = sep_pred_semantics (xs,ys,st,ud,rt,cd);
+
+
+(* ----------------------------------------------------------------------------- *)
+(* CLEANING INSTRUCTION RULES                                                    *)
+(* ----------------------------------------------------------------------------- *)
+
+val reg_rw = prove(
+  ``(!s. s.registers r15 = reg 15w s) /\ 
+    !x s. ~(x = 15w) ==> (REG_READ s.registers (state_mode s) x = reg x s)``,
+  SRW_TAC [] [reg_def]);
+
+val contract_ss = rewrites ([NZCV_def,reg_rw] @ map GSYM
+  [mem_def,status_def,statusN_def,statusZ_def,statusC_def,statusV_def,addr30_def,
+   state_mode_def]);
+
+fun PAT_DISCH tm th = DISCH (hd (filter (can_match tm) (hyp th))) th;
+fun PAT_DISCH_LIST tms th = foldr (uncurry PAT_DISCH) th tms;
+
+fun simple_clean th tms = let
+  val th = SPEC_ALL th
+  val th = INST [``state:arm_mem_state``|->``s:arm_mem_state``] th 
+  val th = INST [``s:bool``|->``s_flag:bool``] th
+  val th = ASM_UNABBREV_ALL_RULE (UD_ALL th)
+  val th = foldr (uncurry DISCH) th tms
+  val th = (UNDISCH_ALL o SIMP_RULE (bool_ss++contract_ss) [] o DISCH_ALL) th
+  val tm1 = ``~s.undefined``
+  val tm2 = ``CONDITION_PASSED2 (status s) c``
+  val tm3 = ``mem (addr30 p) s = enc cmd``
+  val th = PAT_DISCH_LIST ([tm1,tm2,tm3] @ tms) th
+  in th end;
 
 
 (* ----------------------------------------------------------------------------- *)
 (* LDM and STM INSTRUCTIONS                                                      *)
 (* ----------------------------------------------------------------------------- *)
 
-(*
+val _ = Hol_datatype `
+  abbrev_addr4 = am4_DA of bool | am4_IA of bool | am4_DB of bool | am4_IB of bool |
+                 am4_FA of bool | am4_FD of bool | am4_EA of bool | am4_ED of bool`;
 
-(* quick sort *)
+val ADDR_MODE4_CMD_def = Define `
+  (ADDR_MODE4_CMD (am4_DA wb) = <| Pre:=F; Up:=F; BSN:=F; Wb:=wb |>) /\ 
+  (ADDR_MODE4_CMD (am4_FA wb) = <| Pre:=F; Up:=F; BSN:=F; Wb:=wb |>) /\ 
+  (ADDR_MODE4_CMD (am4_IA wb) = <| Pre:=F; Up:=T; BSN:=F; Wb:=wb |>) /\
+  (ADDR_MODE4_CMD (am4_FD wb) = <| Pre:=F; Up:=T; BSN:=F; Wb:=wb |>) /\
+  (ADDR_MODE4_CMD (am4_DB wb) = <| Pre:=T; Up:=F; BSN:=F; Wb:=wb |>) /\
+  (ADDR_MODE4_CMD (am4_EA wb) = <| Pre:=T; Up:=F; BSN:=F; Wb:=wb |>) /\
+  (ADDR_MODE4_CMD (am4_IB wb) = <| Pre:=T; Up:=T; BSN:=F; Wb:=wb |>) /\
+  (ADDR_MODE4_CMD (am4_ED wb) = <| Pre:=T; Up:=T; BSN:=F; Wb:=wb |>)`;
 
-val total_def = Define `total f = !x y. f x y \/ f y x`;
-val transitive_def = Define `transitive f = !x y z. f x y /\ f y z ==> f x z`;
+val NOT_ADDR_MODE4_BSN = prove(
+  ``!x. (ADDR_MODE4_CMD x).BSN = F``,
+  Cases_on `x` \\ SRW_TAC [] [ADDR_MODE4_CMD_def]);
 
-val SORTED_def = Define `
-  (SORTED f  [] = T) /\  
-  (SORTED f [x] = T) /\  
-  (SORTED f (x::y::xs) = f x y /\ SORTED f (y::xs))`;
+val reg_bitmap_def = Define `
+  reg_bitmap (xs:word4 list) = (FCP i. MEM (n2w i) xs):word16`;
 
-val PERM_def = Define `PERM xs ys = !x. FILTER ($= x) xs = FILTER ($= x) ys`;
+val MEM_EQ_EXISTS = prove(
+  ``!xs. MEM x xs = ?ys zs. xs = ys ++ [x] ++ zs``,
+  Induct THEN1 SRW_TAC [] [] 
+  \\ ASM_REWRITE_TAC [MEM] 
+  \\ REPEAT STRIP_TAC \\ EQ_TAC \\ REPEAT STRIP_TAC
+  THEN1 (Q.EXISTS_TAC `[]` \\ Q.EXISTS_TAC `xs` \\ SRW_TAC [] [])
+  THEN1 (Q.EXISTS_TAC `h::ys` \\ Q.EXISTS_TAC `zs` \\ ASM_REWRITE_TAC [APPEND])
+  \\ Cases_on `ys` \\ FULL_SIMP_TAC bool_ss [APPEND,CONS_11] \\ METIS_TAC []);
 
-val PERM_refl = prove(``!xs. PERM xs xs``,METIS_TAC[PERM_def]);
-
-val LENGTH_FILTER_LESS = prove( 
-  ``!xs. LENGTH (FILTER g xs) < SUC (LENGTH xs)``,
-  Induct_on `xs`  
-  \\ SRW_TAC [] [LENGTH,FILTER]
-  \\ METIS_TAC [DECIDE ``!x. x < SUC x``,LESS_TRANS]);
-
-val QSORT_defn = Hol_defn "QSORT" `
-  (QSORT f [] = []) /\
-  (QSORT f (x::xs) = QSORT f (FILTER ($~ o f x) xs) ++ [x] ++
-                     QSORT f (FILTER (f x) xs))`;
-
-val (QSORT_def,QSORT_ind) = Defn.tprove(QSORT_defn,
-  WF_REL_TAC `measure (LENGTH o SND)`
-  \\ METIS_TAC [LENGTH_FILTER_LESS,LENGTH]);
-
-val QSORT_MEM_stable = prove(
-  ``!f xs x. MEM x (QSORT f xs) = MEM x xs``,
-  recInduct QSORT_ind 
-  \\ SIMP_TAC list_ss [QSORT_def,MEM_APPEND,MEM,MEM_FILTER]
-  \\ METIS_TAC []);
-
-val SORTED_eq = prove(
-  ``!f xs x. transitive f
-         ==> (SORTED f (x::xs) = SORTED f xs /\ !y. MEM y xs ==> f x y)``,
-  Induct_on `xs`
-  \\ SRW_TAC [] [SORTED_def,MEM]
-  \\ METIS_TAC [transitive_def]);
-
-val QSORT_perm = prove(
-  ``!f xs. PERM xs (QSORT f xs)``,
-  recInduct QSORT_ind
-  \\ SIMP_TAC list_ss [QSORT_def,PERM_refl,APPEND] 
-  \\ REPEAT STRIP_TAC
-  THEN MATCH_MP_TAC CONS_PERM
-  THEN MATCH_MP_TAC PERM_trans1
-  THEN Q.EXISTS_TAC`APPEND (FILTER(\x. r x h) t) (FILTER(\x. ~r x h) t)`
-  THEN RW_TAC std_ss [BETA_RULE(REWRITE_RULE[o_DEF] PERM_split),PERM_cong]);
-
-val SORTED_APPEND = prove(
-  ``!f xs ys.
-     transitive f /\ SORTED f xs /\ SORTED f ys /\ 
-     (!x y. MEM x xs /\ MEM y ys ==> f x y) ==>
-     SORTED f (APPEND xs ys)``,
-  Induct_on `xs`
-  \\ SIMP_TAC list_ss [MEM] \\ REPEAT STRIP_TAC
-  \\ `SORTED f xs /\ !y. MEM y xs ==> f h y` by PROVE_TAC [SORTED_eq]
-  \\ ASM_SIMP_TAC bool_ss [SORTED_eq] \\ REPEAT STRIP_TAC
-  \\ `MEM y xs \/ MEM y ys` by METIS_TAC [MEM_APPEND]
-  \\ METIS_TAC []);
-
-val QSORT_sorts = prove(
-  ``!f xs. transitive f /\ total f ==> SORTED f (QSORT f xs)``,
-  recInduct QSORT_ind
-  \\ SIMP_TAC list_ss [QSORT_def,SORTED_def]
-  \\ REPEAT STRIP_TAC
-  \\ ONCE_REWRITE_TAC [GSYM APPEND_ASSOC]
-  \\ REWRITE_TAC [APPEND]
-  \\ MATCH_MP_TAC SORTED_APPEND
-  \\ IMP_RES_THEN (fn th => ASM_REWRITE_TAC [th]) SORTED_eq
-  \\ SIMP_TAC list_ss [MEM_FILTER,MEM,QSORT_MEM_stable]
-  \\ METIS_TAC [transitive_def,total_def]);
-
-(* do something better... use Slind's stuff literally *)
-
-val SORTED_LESS = prove(
-  ``!xs:('a word) list. SORTED $<= xs /\ ALL_DISTINCT xs ==> SORTED $< xs``,
-  Induct
-  \\ SRW_TAC [] [ALL_DISTINCT,SORTED_def]
-  \\ Cases_on `xs`
-  \\ SRW_TAC [] [ALL_DISTINCT,SORTED_def]
-  \\ `~(h = h') /\ (h <= h')` by METIS_TAC [SORTED_def,MEM]
-  \\ METIS_TAC [WORD_LESS_OR_EQ,SORTED_def]);
-
-  ``!xs:('a word) list. ALL_DISTINCT xs ==> SORTED $< (QSORT $<= xs)``
-  REPEAT STRIP_TAC
-  MATCH_MP_TAC SORTED_LESS
-
-ALL_DISTINCT
-word_le_def
-
-(* still to come, honestly *)
-
-val ALL_DISTINCT_def = Define `
-  (ALL_DISTINCT [] = T) /\ 
-  (ALL_DISTINCT (x::xs) = ~(MEM x xs) /\ ALL_DISTINCT xs)`;
-
-val GEN_REGLIST_def = Define `
-  GEN_REGLIST (xs:word4 list) = (FCP i. MEM (n2w i) xs):word16`;
-
-val w2n_lt_16 = 
-  SIMP_RULE (std_ss++wordsLib.SIZES_ss) [] (Q.INST_TYPE [`:'a`|->`:i4`] w2n_lt);
-
-val w2n_FCP_BETA = 
-  let
-    val th' = Q.INST_TYPE [`:'a`|->`:i4`] w2n_lt
-    val th' = SIMP_RULE (std_ss++wordsLib.SIZES_ss) [] th'
-    val th = Q.SPEC `w2n (x:word4)` fcpTheory.FCP_BETA
-    val th = Q.INST_TYPE [`:'b`|->`:i16`] th
-    val th = SIMP_RULE (std_ss++wordsLib.SIZES_ss) [] th
-  in
-    MP th (Q.SPEC `x` th')
-  end;
-
-val GEN_REGLIST_MEM = prove(
-  ``!x xs. MEM x xs = GEN_REGLIST xs %% w2n x``,
-  SIMP_TAC std_ss [GEN_REGLIST_def,w2n_FCP_BETA,n2w_w2n]);
-
-val MEM_EQ_LEMMA = prove(
+val MEM_MAP_FILTER = prove(
   ``!x xs. MEM x ((MAP SND o FILTER FST) xs) = MEM (T,x) xs``,        
-  Induct_on `xs`
-  THEN1 SRW_TAC [] [] 
-  \\ Cases_on `h`
-  \\ Cases_on `q`
-  \\ FULL_SIMP_TAC std_ss [FILTER,MAP,MEM]);
+  Induct_on `xs` THEN1 SRW_TAC [] [] 
+  \\ Cases_on `h` \\ Cases_on `q` \\ FULL_SIMP_TAC std_ss [FILTER,MAP,MEM]);
 
-val MEM_EQ_LEMMA2 = prove(
+val MEM_SNOC = prove(
   ``!xs x y. MEM x (SNOC y xs) = MEM x (CONS y xs)``,
   Induct_on `xs` \\ SRW_TAC [] [MEM,SNOC] \\ METIS_TAC []);
 
-val MEM_EQ_LEMMA3 = prove(
-  ``!n x f g. 
-       MEM (T,x) (GENLIST (\i. (f i, g i)) n) = ?i. i < n /\ f i /\ (x = g i)``,
-  Induct
-  THEN1 SIMP_TAC std_ss [MEM,GENLIST]
-  \\ SRW_TAC [] [MEM,GENLIST,MEM_EQ_LEMMA2]
-  \\ Cases_on `f n /\ (x = g n)`
-  \\ ASM_REWRITE_TAC []
+val MEM_GENLIST = prove(
+  ``!n x f. MEM x (GENLIST f n) = ?i. i < n /\ (x = f i)``,
+  Induct THEN1 SIMP_TAC std_ss [MEM,GENLIST]
+  \\ SRW_TAC [] [MEM,GENLIST,MEM_SNOC]
+  \\ Cases_on `x = f n` \\ ASM_REWRITE_TAC []
   THEN1 (Q.EXISTS_TAC `n` \\ SRW_TAC [] [])
   \\ EQ_TAC \\ REPEAT STRIP_TAC << [
-    Q.EXISTS_TAC `i` 
-    \\ METIS_TAC [LESS_TRANS,LESS_EQ_IMP_LESS_SUC,LESS_EQ_REFL],
-    Cases_on `i = n` THEN1 METIS_TAC []
-    \\ `i < n` by DECIDE_TAC \\ METIS_TAC []]);
+    Q.EXISTS_TAC `i` \\ METIS_TAC [LESS_TRANS,LESS_EQ_IMP_LESS_SUC,LESS_EQ_REFL],
+    Cases_on `i = n` THEN1 METIS_TAC [] \\ `i < n` by DECIDE_TAC \\ METIS_TAC []]);
 
-val MEM_EQ_REGISTER_LIST_GEN_REGLIST = prove(
-  ``!x xs. MEM x xs = MEM x (REGISTER_LIST (GEN_REGLIST xs))``,  
+val MEM_PAIR_GENLIST = prove(
+  ``!n x f g. 
+       MEM (T,x) (GENLIST (\i. (f i, g i)) n) = ?i. i < n /\ f i /\ (x = g i)``,
+  SRW_TAC [] [MEM_GENLIST]);
+
+val w2n_FCP_BETA = let
+  val th' = Q.INST_TYPE [`:'a`|->`:i4`] w2n_lt
+  val th' = SIMP_RULE (std_ss++wordsLib.SIZES_ss) [] th'
+  val th = Q.SPEC `w2n (x:word4)` fcpTheory.FCP_BETA
+  val th = Q.INST_TYPE [`:'b`|->`:i16`] th
+  val th = SIMP_RULE (std_ss++wordsLib.SIZES_ss) [] th
+  in MP th (Q.SPEC `x` th') end;
+
+val MEM_reg_bitmap = prove(
+  ``!x xs. MEM x xs = reg_bitmap xs %% w2n x``,
+  SIMP_TAC std_ss [reg_bitmap_def,w2n_FCP_BETA,n2w_w2n]);
+
+val MEM_REGISTER_LIST_reg_bitmap = store_thm("MEM_REGISTER_LIST_reg_bitmap",
+  ``!xs x. MEM x (REGISTER_LIST (reg_bitmap xs)) = MEM x xs``,  
   REPEAT STRIP_TAC
-  \\ REWRITE_TAC [REGISTER_LIST_def,MEM_EQ_LEMMA]
-  \\ REWRITE_TAC [GEN_REGLIST_MEM]
-  \\ REWRITE_TAC [MEM_EQ_LEMMA3]
-  \\ EQ_TAC \\ STRIP_TAC
-  THEN1 (Q.EXISTS_TAC `w2n (x:word4)` \\ SRW_TAC [] [n2w_w2n,w2n_lt_16])
-  \\ ASM_SIMP_TAC (std_ss++wordsLib.SIZES_ss) [w2n_n2w]);
+  \\ REWRITE_TAC [REGISTER_LIST_def,MEM_MAP_FILTER]
+  \\ REWRITE_TAC [MEM_reg_bitmap]
+  \\ REWRITE_TAC [MEM_PAIR_GENLIST]
+  \\ ASSUME_TAC (Q.INST_TYPE [`:'a`|->`:i4`] w2n_lt)
+  \\ EQ_TAC \\ STRIP_TAC \\ FULL_SIMP_TAC (std_ss++wordsLib.SIZES_ss) [w2n_n2w]
+  \\ Q.EXISTS_TAC `w2n (x:word4)` \\ FULL_SIMP_TAC (std_ss++wordsLib.SIZES_ss) [n2w_w2n]);
 
-val MEM_IMP_SPLIT = prove(   
-  ``!ys y. MEM y ys ==> ?zs zs'. ys = zs ++ [y] ++ zs'``,
+val SNOC_CONS = prove(
+  ``!xs x y. SNOC x (y::xs) = y::(SNOC x xs)``,Induct \\ ASM_REWRITE_TAC [SNOC]);
+  
+val FILTER_SNOC = prove(
+  ``!xs x P. FILTER P (SNOC x xs) = if P x then SNOC x (FILTER P xs) else FILTER P xs``,  
+  Induct \\ ASM_REWRITE_TAC [SNOC,FILTER] \\ SRW_TAC [] [SNOC_CONS]);
+
+val MAP_SNOC = prove(
+  ``!xs x f. MAP f (SNOC x xs) = SNOC (f x) (MAP f xs)``,
+  Induct \\ ASM_REWRITE_TAC [SNOC,MAP] \\ SRW_TAC [] [SNOC_CONS]);
+    
+val SORTED_SNOC_SNOC = prove(
+  ``!xs f x y. SORTED f (SNOC x (SNOC y xs)) = f y x /\ SORTED f (SNOC y xs)``,
+  Induct \\ FULL_SIMP_TAC std_ss [SNOC,SORTED_DEF]
+  \\ REPEAT STRIP_TAC \\ Cases_on `xs`
+  \\ FULL_SIMP_TAC std_ss [SNOC,SORTED_DEF] \\ METIS_TAC []);
+
+val SORTED_REGISTER_LIST_LEMMA = prove(
+  ``!k g:word16. 
+      k <= 16 ==> 
+      SORTED $<+ ((MAP SND o FILTER FST) (GENLIST (\i. (g %% i,(n2w i):word4)) k))``,
   Induct 
-  THEN1 SRW_TAC [] []
-  \\ REPEAT STRIP_TAC
-  \\ Cases_on `y = h` << [
-    Q.EXISTS_TAC `[]` 
-    \\ Q.EXISTS_TAC `ys` 
-    \\ ASM_SIMP_TAC std_ss [APPEND],
-    FULL_SIMP_TAC std_ss [MEM]
-    \\ `?zs zs'. ys = zs ++ [y] ++ zs'` by METIS_TAC []
-    \\ Q.EXISTS_TAC `h::zs`
-    \\ Q.EXISTS_TAC `zs'`
-    \\ ASM_SIMP_TAC std_ss [APPEND]]);
+  \\ SIMP_TAC std_ss [GENLIST,FILTER,MAP,SORTED_DEF,FILTER_SNOC]
+  \\ REPEAT STRIP_TAC \\ Cases_on `g %% k` 
+  \\ `k <= 16` by DECIDE_TAC
+  \\ PAT_ASSUM ``!g'. b`` (ASSUME_TAC o UNDISCH o Q.SPEC `g`)
+  \\ FULL_SIMP_TAC std_ss [MAP_SNOC]
+  \\ STRIP_ASSUME_TAC (Q.ISPEC `MAP SND (FILTER FST 
+       (GENLIST (\i. ((g:word16) %% i,((n2w i):word4))) k))` SNOC_CASES)
+  \\ FULL_SIMP_TAC std_ss [SNOC,SORTED_DEF,SORTED_SNOC_SNOC]
+  \\ `!xs. MEM x (SNOC x xs)` by (Induct \\ SRW_TAC [] [MEM,SNOC])
+  \\ `MEM x (MAP SND (FILTER FST (GENLIST (\i. (g %% i,n2w i)) k)))` by METIS_TAC [] 
+  \\ FULL_SIMP_TAC std_ss [MEM_MAP,MEM_FILTER,MEM_GENLIST]
+  \\ `k < 16 /\ i < 16` by DECIDE_TAC
+  \\ ASM_SIMP_TAC (std_ss++wordsLib.SIZES_ss) [word_lo_n2w]);
 
-val rs_def = Define `
-  (rs [] = emp) /\ 
-  (rs ((r,x)::xs) = R r x * rs xs)`;
+val SORTED_REGISTER_LIST = store_thm("SORTED_REGSITER_LIST",
+  ``!g. SORTED $<+ (REGISTER_LIST g)``,
+  REWRITE_TAC [REGISTER_LIST_def]
+  \\ MATCH_MP_TAC (SPEC_ALL SORTED_REGISTER_LIST_LEMMA) \\ DECIDE_TAC);
 
-val rs'_def = Define `
-  (rs' [] = emp) /\ 
-  (rs' ((r,x)::xs) = ~ (R r) * rs' xs)`;
-
-val ms_def = Define `
-  (ms a [] = emp) /\
-  (ms a (x::xs) = M (addr30 a) x * ms (a+4w:word32) xs)`;
-
-val ms'_def = Define `
-  (ms' a [] = emp) /\
-  (ms' a (x::xs) = ~ (M (addr30 a)) * ms' (a+4w:word32) xs)`;
-
-val LENGTH_FILTER_LESS = prove( 
-  ``!xs. LENGTH (FILTER g xs) < SUC (LENGTH xs)``,
-  Induct_on `xs`  
-  \\ SRW_TAC [] [LENGTH,FILTER]
-  \\ METIS_TAC [DECIDE ``!x. x < SUC x``,LESS_TRANS]);
-
-val QSORT_defn = Hol_defn "QSORT" `
-  (QSORT f [] = []) /\
-  (QSORT f (x::xs) = QSORT f (FILTER ($~ o f x) xs) ++ [x] ++
-                     QSORT f (FILTER (f x) xs))`;
-
-val (QSORT_def,QSORT_ind) = Defn.tprove(QSORT_defn,
-  WF_REL_TAC `measure (LENGTH o SND)`
-  \\ METIS_TAC [LENGTH_FILTER_LESS,LENGTH]);
-
-val SORTED_def = Define `
-  SORTED f xs = !ys y z zs. (xs = ys ++ [y;z] ++ zs) ==> f y z`;
-
-val SORTED_QSORT_LEMMA = prove(
- ``!xs g. ALL_DISTINCT xs ==> ALL_DISTINCT (FILTER g xs)``,
-  Induct \\ SRW_TAC [] [ALL_DISTINCT_def]
-  \\ `~MEM h xs ==> ~MEM h (FILTER g xs)` by ALL_TAC << [
-    POP_ASSUM_LIST (fn thms => ALL_TAC)
-    \\ Induct_on `xs` \\ SRW_TAC [] [MEM,FILTER],
-    METIS_TAC []]);
-
-val MEM_FILTER_IMP = prove(
-  ``!xs x g. MEM x (FILTER g xs) ==> MEM x xs``,
-  Induct \\ SRW_TAC [] [] \\ METIS_TAC []);
-
-val SAME_PREFIX = prove(
-  ``!xs ys zs zs'. (LENGTH xs = LENGTH ys) /\ (xs ++ zs = ys ++ zs') ==> (xs = ys)``,
-  Induct THEN1 METIS_TAC [LENGTH_NIL,LENGTH]
-  \\ SRW_TAC [] [LENGTH]
-  \\ `?h' ys'. (LENGTH xs = LENGTH ys') /\ (ys = h'::ys')` by METIS_TAC [LENGTH_CONS]
-  \\ FULL_SIMP_TAC std_ss [APPEND,CONS_11]
+val SORTED_CONS_IMP = prove(
+  ``!xs h. SORTED $<+ (h::xs) ==> SORTED $<+ xs /\ ~(MEM h xs) /\ EVERY (\x. h <+ x) xs``,
+  Induct \\ SRW_TAC [] [MEM,SORTED_DEF] THEN1 METIS_TAC [WORD_NOT_LOWER_EQ]
+  \\ `SORTED $<+ (h'::xs)` by (Cases_on `xs` \\ METIS_TAC [SORTED_DEF,WORD_LOWER_TRANS])
   \\ METIS_TAC []);
 
-  ``!xs:'a word list h ys. 
-      SORTED $< xs /\ SORTED $< ys /\ 
-      (!x. MEM x xs ==> x < h) /\ (!y. MEM y ys ==> h < y) ==> 
-      SORTED $< (xs ++ [h] ++ ys)``,
-  REWRITE_TAC [SORTED_def]
-  REPEAT STRIP_TAC
-  Cases_on `LENGTH xs = LENGTH ys'`
-
-    `xs = ys'` by METIS_TAC [SAME_PREFIX,APPEND_ASSOC]
-    \\ FULL_SIMP_TAC std_ss [APPEND_11,GSYM APPEND_ASSOC]
-    \\ Cases_on `ys`
-    \\ FULL_SIMP_TAC bool_ss [APPEND]    
-
-      open listTheory;
-    
-
-val SORTED_QSORT = prove(
-  ``!xs:'a word list. 
-       ALL_DISTINCT xs ==> 
-       SORTED $< (QSORT $< xs) /\ (!x. MEM x xs = MEM x (QSORT $< xs))``,
-  STRIP_TAC \\ completeInduct_on `LENGTH xs` \\ Cases_on `v`
-
-    REPEAT STRIP_TAC
-    \\ `xs = []` by METIS_TAC [LENGTH_NIL]
-    \\ SRW_TAC [] [QSORT_def,SORTED_def]
-
-    NTAC 3 STRIP_TAC
-    \\ `?h xs'. (LENGTH xs' = n) /\ (xs = h::xs')` by METIS_TAC [LENGTH_CONS]
-    \\ ASM_REWRITE_TAC [QSORT_def]
-    \\ `LENGTH (FILTER ($~ o $< h) xs') < SUC n` by METIS_TAC [LENGTH_FILTER_LESS] 
-    \\ `LENGTH (FILTER ($< h) xs') < SUC n` by METIS_TAC [LENGTH_FILTER_LESS]    
-    \\ `ALL_DISTINCT xs'` by METIS_TAC [ALL_DISTINCT_def]
-    \\ `ALL_DISTINCT (FILTER ($~ o $< h) xs')` by METIS_TAC [SORTED_QSORT_LEMMA]
-    \\ `ALL_DISTINCT (FILTER ($< h) xs')` by METIS_TAC [SORTED_QSORT_LEMMA]
-    \\ STRIP_TAC
-      
-      `SORTED $< (QSORT $< (FILTER ($~ o $< h) xs'))` by METIS_TAC []
-      \\ `SORTED $< (QSORT $< (FILTER ($< h) xs'))` by METIS_TAC []
-      
-      REWRITE_TAC [MEM_APPEND,MEM] 
-      \\ REPEAT STRIP_TAC 
-      \\ EQ_TAC << [
-        STRIP_TAC \\ Cases_on `x = h` \\ ASM_REWRITE_TAC []      
-        THEN1 METIS_TAC []      
-        \\ `(($< h) x) \/ (($~ o $< h) x)` by SRW_TAC [] []      
-        \\ METIS_TAC [MEM_FILTER],
-        METIS_TAC [MEM_FILTER_IMP]]
-        
-        
-
-val REGSORT_def = Define `
-  (REGSORT:(word4#word32) list->(word4#word32) list) = QSORT (\x y. FST x < FST y)`;
-
-val MBLOCK_WB_def = Define `
-  MBLOCK_WB wb U base xs = 
-    if wb then WB_ADDRESS U base (LENGTH xs) else base`;
-
-val MBLOCK_ADDR_def = Define `
-  MBLOCK_ADDR P U base xs = 
-    FIRST_ADDRESS P U base (MBLOCK_WB T U base xs)`;
-
-val MBLOCK_def = Define `
-  MBLOCK P U base xs = ms (MBLOCK_ADDR P U base xs) (MAP SND (REGSORT xs))`;
-
-
-val MAP_FST_REGSORT_LEMMA = prove(
-  ``!xs f h. FILTER f (MAP FST xs) = MAP FST (FILTER (\y. f (FST y)) xs)``,
-  Induct 
-  \\ SRW_TAC [] []
-  \\ FULL_SIMP_TAC std_ss []);
-
-val MAP_FST_REGSORT = prove(
-  ``!xs. MAP FST (REGSORT xs) = QSORT ($<) (MAP FST xs)``,
-  STRIP_TAC
-  \\ completeInduct_on `LENGTH xs`
-  \\ Cases_on `v`
-  \\ REPEAT STRIP_TAC << [    
-    `xs = []` by METIS_TAC [LENGTH_NIL]
-    \\ ASM_SIMP_TAC std_ss [REGSORT_def,MAP,QSORT_def],
-    `?h xs'. (LENGTH xs' = n) /\ (xs = h::xs')` by METIS_TAC [LENGTH_CONS]
-    \\ ASM_REWRITE_TAC [QSORT_def,REGSORT_def]
-    \\ Cases_on `h`
-    \\ FULL_SIMP_TAC bool_ss [REGSORT_def,MAP_APPEND,MAP,QSORT_def]
-    \\ REWRITE_TAC [MAP_FST_REGSORT_LEMMA]
-    \\ FULL_SIMP_TAC std_ss []
-    \\ `LENGTH (FILTER (\y. ~(q < FST y)) xs') < SUC n` by METIS_TAC [LENGTH_FILTER_LESS] 
-    \\ `LENGTH (FILTER (\y. q < FST y) xs') < SUC n` by METIS_TAC [LENGTH_FILTER_LESS]    
-    \\ METIS_TAC []]);
-
-
-(*
-
-  ``!ys xs h. 
-      ALL_DISTINCT xs /\ ALL_DISTINCT ys /\ 
-      SORTED f xs /\ SORTED f ys /\ (!x. MEM x xs ==> f x h) ==> 
-      SORTED f (ISORT_INSERT f h xs ys)``
-  Induct
-
-    REWRITE_TAC [ISORT_INSERT_def]
-    \\ REWRITE_TAC [SORTED_def]
-    \\ REPEAT STRIP_TAC        
-    \\ Cases_on `zs`    
-
-
-val SORTED_ISORT' = prove(
-  ``!f xs ys. ALL_DISTINCT xs /\ SORTED f ys ==> SORTED f (ISORT' f xs ys)``,
-  Induct_on `xs`
-  THEN1 SRW_TAC [] [ISORT'_def]
-
-  ``!f xs. ALL_DISTINCT xs ==> SORTED f (ISORT f xs)``
-  STRIP_TAC
-  \\ REWRITE_TAC [ISORT_def]
-  \\ `!xs ys. ALL_DISTINCT xs /\ SORTED f ys ==> SORTED f (ISORT' f xs ys)` by ALL_TAC
-
-    Induct THEN1 SRW_TAC [] [ISORT'_def]
-    `!ys xs h. 
-       SORTED f xs /\ SORTED f ys /\ (!x. MEM x xs ==> f x h) ==> 
-       SORTED f (ISORT_INSERT f h xs ys)` by ALL_TAC
-
-      Induct 
-
-        REWRITE_TAC [ISORT_INSERT_def]
-        REPEAT STRIP_TAC        
-        REWRITE_TAC [SORTED_def]
-
-*)
-
-
-val SORTED_TRANS = prove(
-  ``!xs f h h' ys.
-      (!x y z. f x y /\ f y z ==> f x z) /\ 
-      SORTED f (h::xs ++ [h'] ++ ys) ==> f h h'``,
-  Induct THEN1 METIS_TAC [SORTED_def,APPEND]
-  \\ REPEAT STRIP_TAC
-  \\ `h'::h::xs ++ [h''] ++ ys = [] ++ [h';h]++ (xs ++ [h''] ++ ys)` by METIS_TAC [APPEND]
-  \\ `f h' h` by METIS_TAC [SORTED_def]
-  \\ `!x xs. SORTED f (x::xs) ==> SORTED f xs` by METIS_TAC [SORTED_def,APPEND]
-  \\ METIS_TAC [APPEND]);
-
-val SORTED_IMP_EQ = prove(
-  ``!f xs ys.
-      (!x y z. f x y /\ f y z ==> f x z) /\ (!x y. ~(f x y /\ f y x)) /\ 
-      SORTED f xs /\ SORTED f ys /\
-      (!x. MEM x xs = MEM x ys) ==> (xs = ys)``,
-  STRIP_TAC
-  \\ Induct 
-  THEN1 METIS_TAC [MEM]
-  \\ REPEAT STRIP_TAC  
+val SORTED_LO_IMP_EQ = store_thm("SORTED_LOWER_IMP_EQ",
+  ``!xs ys. SORTED $<+ xs /\ SORTED $<+ ys /\ (!x. MEM x xs = MEM x ys) ==> (xs = ys)``,
+  Induct THEN1 (Cases_on `ys` \\ SRW_TAC [] [MEM] \\ METIS_TAC [])
+  \\ REWRITE_TAC [MEM] \\ REPEAT STRIP_TAC 
   \\ `MEM h ys` by METIS_TAC []
-  \\ `?zs zs'. ys = zs ++ [h] ++ zs'` by METIS_TAC [MEM_IMP_SPLIT]
-  \\ Cases_on `zs` << [
-    ASM_REWRITE_TAC [APPEND]
-    \\ `!x xs. SORTED f (x::xs) ==> SORTED f xs` by METIS_TAC [SORTED_def,APPEND]
-    \\ METIS_TAC [],
-    `MEM h' (h::xs)` by METIS_TAC [MEM]
-    \\ Cases_on `h = h'` THEN1 METIS_TAC [ALL_DISTINCT_def,MEM]
-    \\ `MEM h' xs` by METIS_TAC [MEM]
-    \\ `?zs1 zs1'. xs = zs1 ++ [h'] ++ zs1'` by METIS_TAC [MEM_IMP_SPLIT]
-    \\ `f h h'` by METIS_TAC [SORTED_TRANS]
-    \\ `f h' h` by METIS_TAC [SORTED_TRANS]
-    \\ METIS_TAC []]);
+  \\ `?hs zs. ys = hs ++ [h] ++ zs` by METIS_TAC [MEM_EQ_EXISTS]
+  \\ Q.PAT_ASSUM `!ys. b ==> (c:bool)` (ASSUME_TAC o Q.SPEC `zs`)
+  \\ Cases_on `hs` \\ FULL_SIMP_TAC std_ss [CONS_11,APPEND,MEM]
+  THEN1 METIS_TAC [SORTED_CONS_IMP]
+  \\ IMP_RES_TAC SORTED_CONS_IMP
+  \\ FULL_SIMP_TAC std_ss [MEM_APPEND,MEM,EVERY_APPEND,EVERY_DEF]
+  \\ `MEM h' xs` by METIS_TAC []
+  \\ `?hs' zs'. xs = hs' ++ [h'] ++ zs'` by METIS_TAC [MEM_EQ_EXISTS]
+  \\ FULL_SIMP_TAC std_ss [EVERY_APPEND,EVERY_DEF] \\ METIS_TAC [WORD_LOWER_ANTISYM]);
 
 
-  ``ALL_DISTINCT (MAP FST ys) ==>
-    (FST (ADDR_MODE4 P U x (GEN_REGLIST (MAP FST ys))) = MAP FST (REGSORT ys))``
-  SIMP_TAC std_ss [ADDR_MODE4_def,LET_DEF]
-  \\ REWRITE_TAC [MAP_FST_REGSORT]
-  \\ Q.ABBREV_TAC `x = MAP FST ys`  
-
-  WORD_LESS_TRANS
-  WORD_LESS_ANTISYM
-
-  Q.SPEC `$<:word4->word4->bool` (Q.INST_TYPE [`:'a`|->`:word4`] SORTED_IMP_EQ)
-
-  MEM_EQ_REGISTER_LIST_GEN_REGLIST
-  Q.ISPEC `$<:word4->word4->bool` SORTED_QSORT
-
-show_types := false
-show_types_verbosely := false
-
-(*
-
-  target specs, sketches only:
-
-  STM pre:    R a x * rs ys * MBLOCK' P U x ys * cond ~(ys = [])
-  STM post:   R a (MBLOCK_WB wb U x ys) * rs ys * MBLOCK P U x ys
-
-  LDM pre:    R a x * rs' ys * MBLOCK P U x ys * cond ~(ys = [])
-  LDM post:   R a (MBLOCK_WB wb U x ys) * rs ys * MBLOCK P U x ys
-
-*)
 
 
-ADDR_MODE4_def
-REGISTER_LIST_def
-WB_ADDRESS_def
-FIRST_ADDRESS_def
-ADDRESS_LIST_def
-GENLIST
+val LEAST_MEM_def = Define `
+  (LEAST_MEM [x] = x) /\ 
+  (LEAST_MEM (x::y::ys) = 
+     let m = LEAST_MEM (y::ys) in if x <=+ m then x else m)`;
 
-    val th = ARM_LDM
-    val th = SPEC_ALL th
-    val th = DISCH_ALL (ASM_UNABBREV_ALL_RULE (UD_ALL th))
-    val th = RW [GSYM state_mode_def] th
-    val th = Q.INST [`opt`|->`<| Pre:=P; Up:=U; BSN:=F; Wb:=wb |>`] th
-    val th = DISCH ``~(Rd:word4 = 15w)`` th
-    val th = SIMP_RULE (srw_ss()) [] th
-    val th = Q.INST [`list`|->`GEN_REGLIST (MAP FST ys)`] th
+val LENGTH_FILTER = prove(
+  ``!xs P. LENGTH (FILTER P xs) <= LENGTH xs ``,
+  Induct \\ SIMP_TAC std_ss [FILTER,LENGTH] \\ REPEAT STRIP_TAC
+  \\ Cases_on `P h` \\ ASM_REWRITE_TAC [LENGTH] 
+  \\ PAT_ASSUM ``!P:'a. b:bool`` (ASSUME_TAC o SPEC_ALL) \\ DECIDE_TAC );
 
-    val th = Q.INST [`list`|->`3w:word16`] th
+val LEAST_SORT_LEMMA = prove(
+  ``!xs m. MEM m xs ==> LENGTH (FILTER (\x. ~(x = m)) xs) < LENGTH xs``,
+  Induct THEN1 SRW_TAC [] []
+  \\ SIMP_TAC std_ss [MEM,FILTER,LENGTH] \\ NTAC 2 STRIP_TAC
+  \\ Cases_on `h = m` \\ ASM_REWRITE_TAC [LESS_EQ,DECIDE ``n < SUC m = n <= m``]
+  THEN1 METIS_TAC [LENGTH_FILTER,LESS_LESS_EQ_TRANS]
+  \\ `~(m = h)` by METIS_TAC [] \\ ASM_REWRITE_TAC [LENGTH,GSYM LESS_EQ]);
 
-*)
+val MEM_LEAST_MEM = prove(
+  ``!xs x. MEM (LEAST_MEM (x::xs)) (x::xs)``,
+  Induct \\ ONCE_REWRITE_TAC [LEAST_MEM_def] \\ SIMP_TAC std_ss [LET_DEF]
+  THEN1 REWRITE_TAC [MEM]
+  \\ Cases_on `x <=+ LEAST_MEM (h::xs)` \\ ASM_REWRITE_TAC []
+  THEN1 REWRITE_TAC [MEM] \\ ONCE_REWRITE_TAC [MEM] \\ ASM_REWRITE_TAC []);
+
+val (LEAST_SORT_def,LEAST_SORT_ind) = let
+  val d = Defn.Hol_defn "LEAST_SORT" `
+    (LEAST_SORT [] = []) /\
+    (LEAST_SORT (x::xs) = 
+       let m = LEAST_MEM (x::xs) in 
+         m :: LEAST_SORT (FILTER (\x. ~(x = m)) (x::xs)))`
+  val tac = WF_REL_TAC `measure LENGTH` \\ METIS_TAC [LEAST_SORT_LEMMA,MEM_LEAST_MEM,MEM]
+  in Defn.tprove (d,tac) end;
+
+val MEM_LEAST_SORT = prove(
+  ``!xs x. MEM x (LEAST_SORT xs) = MEM x xs``,
+  recInduct LEAST_SORT_ind \\ REWRITE_TAC [LEAST_SORT_def] \\ REPEAT STRIP_TAC
+  \\ SIMP_TAC std_ss [LET_DEF]
+  \\ Cases_on `x' = LEAST_MEM (x::xs)`
+  THEN1 (ASM_REWRITE_TAC [MEM_LEAST_MEM] \\ REWRITE_TAC [MEM])
+  \\ CONV_TAC (RATOR_CONV (REWRITE_CONV [MEM])) \\ ASM_REWRITE_TAC []
+  \\ Q.PAT_ASSUM `!m. b:bool` 
+       (ASSUME_TAC o Q.SPEC `x'` o REWRITE_RULE [] o Q.SPEC `LEAST_MEM (x::xs)`)
+  \\ ASM_SIMP_TAC std_ss [MEM_FILTER]);
+
+val SORTED_EQ_LOWER = 
+  (REWRITE_RULE [relationTheory.transitive_def,WORD_LOWER_TRANS] o Q.ISPEC `$<+`) SORTED_EQ;
+
+val LEAST_MEM_IMP = prove(
+  ``!xs x y. (y = LEAST_MEM (x::xs)) ==> !z. MEM z (x::xs) ==> (y = z) \/ (y <+ z)``,
+  Induct \\ REWRITE_TAC [LEAST_MEM_def,MEM] THEN1 METIS_TAC []
+  \\ SIMP_TAC std_ss [LET_DEF] \\ NTAC 3 STRIP_TAC
+  \\ POP_ASSUM (ASSUME_TAC o REWRITE_RULE [] o Q.SPECL [`h`,`LEAST_MEM (h::xs)`])    
+  \\ Cases_on `z = x` \\ ASM_SIMP_TAC bool_ss []
+  \\ Cases_on `x <=+ LEAST_MEM (h::xs)` \\ ASM_REWRITE_TAC []
+  THEN1 METIS_TAC [WORD_LOWER_CASES]
+  \\ FULL_SIMP_TAC std_ss [MEM,WORD_LOWER_OR_EQ]
+  \\ METIS_TAC [WORD_LOWER_TRANS]);
+
+val LEAST_MEM_LOWER_EQ = prove(
+  ``!xs x. MEM x xs ==> LEAST_MEM xs <=+ x``,
+  Induct \\ SIMP_TAC std_ss [MEM,LEAST_MEM_def]
+  \\ Cases_on `xs` \\ SIMP_TAC std_ss [LEAST_MEM_def,LET_DEF]
+  THEN1 SRW_TAC [] [MEM,WORD_LOWER_EQ_REFL] \\ NTAC 2 STRIP_TAC
+  \\ Cases_on `x = h'` \\ ASM_REWRITE_TAC []
+  THEN1 METIS_TAC [WORD_LOWER_EQ_CASES]
+  \\ Cases_on `h' <=+ LEAST_MEM (h::t)` \\ ASM_REWRITE_TAC []
+  \\ METIS_TAC [WORD_LOWER_EQ_TRANS]);
+
+val SORTED_LEAST_SORT = prove(
+  ``!xs. SORTED $<+ (LEAST_SORT xs)``,
+  recInduct LEAST_SORT_ind \\ SIMP_TAC std_ss 
+    [LEAST_SORT_def,LET_DEF,SORTED_DEF,SORTED_EQ_LOWER,MEM_LEAST_SORT,MEM_FILTER]
+  \\ REPEAT STRIP_TAC \\ IMP_RES_TAC LEAST_MEM_LOWER_EQ
+  \\ FULL_SIMP_TAC std_ss [WORD_LOWER_OR_EQ] \\ METIS_TAC [WORD_LOWER_REFL]);
+
+val REGISTER_LIST_EQ_LEAST_SORT = prove(
+  ``!xs. REGISTER_LIST (reg_bitmap xs) = LEAST_SORT xs``,
+  STRIP_TAC \\ MATCH_MP_TAC SORTED_LO_IMP_EQ
+  \\ REWRITE_TAC [MEM_REGISTER_LIST_reg_bitmap,MEM_LEAST_SORT,
+                  SORTED_LEAST_SORT,SORTED_REGISTER_LIST]);
+
+val ALL_DISTINCT_FILTER = prove(
+  ``!xs. ALL_DISTINCT xs ==> !g. ALL_DISTINCT (FILTER g xs)``,
+  Induct \\ REWRITE_TAC [ALL_DISTINCT,FILTER] \\ REPEAT STRIP_TAC
+  \\ Cases_on `g h` \\ ASM_REWRITE_TAC [ALL_DISTINCT,MEM_FILTER] \\ METIS_TAC []);
+
+val LENGTH_FILTER_NEQ = prove(
+  ``!xs y. ALL_DISTINCT xs /\ MEM y xs ==> 
+           (LENGTH (FILTER (\x. ~(x = y)) xs) = LENGTH xs - 1)``,
+  Induct \\ SIMP_TAC bool_ss [MEM,FILTER,ALL_DISTINCT]
+  \\ NTAC 2 STRIP_TAC \\ Cases_on `y = h` \\ ASM_REWRITE_TAC [LENGTH]
+  \\ `!xs. ~MEM h xs ==> (FILTER (\x. ~(x = h)) xs = xs)` by (Induct \\ SRW_TAC [] [FILTER])
+  \\ ASM_SIMP_TAC std_ss [ADD1,ADD_SUB,LENGTH]
+  \\ Cases_on `xs` \\ REWRITE_TAC [MEM,LENGTH,ADD1,ADD_SUB]);
+
+val LENGTH_LEAST_SORT = prove(
+  ``!xs. ALL_DISTINCT xs ==> (LENGTH (LEAST_SORT xs) = LENGTH xs)``,
+  recInduct LEAST_SORT_ind \\ SIMP_TAC std_ss [LENGTH,LEAST_SORT_def,LET_DEF]
+  \\ REPEAT STRIP_TAC \\ IMP_RES_TAC ALL_DISTINCT_FILTER
+  \\ Q.PAT_ASSUM `!g.b:bool` (ASSUME_TAC o Q.SPEC `\x'. ~(x' = LEAST_MEM (x::xs))`)
+  \\ FULL_SIMP_TAC bool_ss [] 
+  \\ ASSUME_TAC (Q.SPECL [`xs`,`x`] MEM_LEAST_MEM)
+  \\ IMP_RES_TAC LENGTH_FILTER_NEQ \\ ASM_REWRITE_TAC [LENGTH,ADD1,ADD_SUB]);
+
+
+val PERM_IMP_MEM_EQUALITY = prove(
+  ``!xs ys. PERM xs ys ==> !x. MEM x xs = MEM x ys``,
+  REPEAT STRIP_TAC
+  \\ `!xs. MEM x xs = ~(FILTER ($= x) xs = [])` by (Induct \\ SRW_TAC [] [MEM,FILTER])
+  \\ FULL_SIMP_TAC bool_ss [PERM_DEF]);
+
+val ALL_DISTINCT_MOVE_CONS = prove(
+  ``!xs ys. ALL_DISTINCT (xs ++ h::ys) = ALL_DISTINCT (h::xs ++ ys)``,
+  Induct \\ ASM_SIMP_TAC bool_ss [APPEND,APPEND_NIL] \\ REPEAT STRIP_TAC
+  \\ ASM_REWRITE_TAC [ALL_DISTINCT,APPEND,MEM_APPEND,MEM]
+  \\ REPEAT STRIP_TAC \\ EQ_TAC \\ REPEAT STRIP_TAC \\ FULL_SIMP_TAC std_ss []);
+
+val PERM_ALL_DISTINCT = prove(
+  ``!xs ys. ALL_DISTINCT xs /\ PERM xs ys ==> ALL_DISTINCT ys``,
+  Induct \\ SIMP_TAC bool_ss [PERM_NIL,ALL_DISTINCT,PERM_CONS_EQ_APPEND]
+  \\ REPEAT STRIP_TAC \\ ASM_REWRITE_TAC [] \\ IMP_RES_TAC PERM_IMP_MEM_EQUALITY
+  \\ REWRITE_TAC [ALL_DISTINCT_MOVE_CONS,ALL_DISTINCT,APPEND] \\ METIS_TAC []);
+
+val QSORT_SORTS_LS = prove(
+  ``SORTS QSORT ($<=+ :'a word->'a word->bool)``,
+  MATCH_MP_TAC QSORT_SORTS
+  \\ REWRITE_TAC [transitive_def,total_def,WORD_LOWER_EQ_TRANS,WORD_LOWER_EQ_CASES]);
+
+val SORTED_LO = prove(
+  ``!xs. SORTED $<=+ xs /\ ALL_DISTINCT xs ==> SORTED $<+ (xs:'a word list)``,
+  Induct \\ REWRITE_TAC [SORTED_DEF]
+  \\ Cases_on `xs` \\ REWRITE_TAC [SORTED_DEF]
+  \\ ONCE_REWRITE_TAC [ALL_DISTINCT]
+  \\ REWRITE_TAC [MEM] \\ METIS_TAC [WORD_LOWER_OR_EQ]);
+
+val ADDR_MODE4_UP_def = Define `
+  (ADDR_MODE4_UP (am4_DA wb) = F) /\ 
+  (ADDR_MODE4_UP (am4_FA wb) = F) /\ 
+  (ADDR_MODE4_UP (am4_IA wb) = T) /\
+  (ADDR_MODE4_UP (am4_FD wb) = T) /\
+  (ADDR_MODE4_UP (am4_DB wb) = F) /\
+  (ADDR_MODE4_UP (am4_EA wb) = F) /\
+  (ADDR_MODE4_UP (am4_IB wb) = T) /\
+  (ADDR_MODE4_UP (am4_ED wb) = T)`;
+
+val ADDR_MODE4_wb_def = Define `
+  (ADDR_MODE4_wb (am4_DA wb) = wb) /\ 
+  (ADDR_MODE4_wb (am4_FA wb) = wb) /\ 
+  (ADDR_MODE4_wb (am4_IA wb) = wb) /\
+  (ADDR_MODE4_wb (am4_FD wb) = wb) /\
+  (ADDR_MODE4_wb (am4_DB wb) = wb) /\
+  (ADDR_MODE4_wb (am4_EA wb) = wb) /\
+  (ADDR_MODE4_wb (am4_IB wb) = wb) /\
+  (ADDR_MODE4_wb (am4_ED wb) = wb)`;
+
+val ADDR_MODE4_WB'_def = Define `
+  ADDR_MODE4_WB' am4 x n = 
+    (if ADDR_MODE4_UP am4 then $+ else $-) x (n2w n)`;
+
+val ADDR_MODE4_WB_def = Define `
+  ADDR_MODE4_WB am4 x xs = 
+    if ADDR_MODE4_wb am4 then ADDR_MODE4_WB' am4 x (LENGTH xs) else x`;
+
+val ALL_DISTINCT_IMP_LENGTH_EQ = prove(
+  ``!xs ys. ALL_DISTINCT xs /\ ALL_DISTINCT ys /\ (!x. MEM x xs = MEM x ys) ==>
+            (LENGTH xs = LENGTH ys)``,
+  Induct THEN1 (Cases_on `ys` \\ SRW_TAC [] [] \\ METIS_TAC [])
+  \\ REWRITE_TAC [MEM] \\ REPEAT STRIP_TAC
+  \\ `MEM h ys` by METIS_TAC []
+  \\ `?hs zs. ys = hs ++ [h] ++ zs` by METIS_TAC [MEM_EQ_EXISTS]
+  \\ FULL_SIMP_TAC std_ss [GSYM APPEND_ASSOC,APPEND,ALL_DISTINCT_MOVE_CONS,MEM,MEM_APPEND]
+  \\ FULL_SIMP_TAC bool_ss [ALL_DISTINCT,MEM_APPEND,LENGTH,LENGTH_APPEND]
+  \\ `!x. MEM x xs = MEM x (hs ++ zs)` by METIS_TAC [MEM_APPEND]
+  \\ Q.PAT_ASSUM `!ys'. b ==> (c:bool)` IMP_RES_TAC  
+  \\ ASM_REWRITE_TAC [ADD1,LENGTH_APPEND] \\ DECIDE_TAC);
+
+val SORTED_LO_IMP_ALL_DISTINCT = prove(
+  ``!xs. SORTED $<+ xs ==> ALL_DISTINCT xs``,
+  Induct \\ REWRITE_TAC [SORTED_DEF,ALL_DISTINCT]
+  \\ REPEAT STRIP_TAC \\ IMP_RES_TAC SORTED_CONS_IMP \\ METIS_TAC []);
+
+val REGISTER_LIST_LENGTH = prove(
+  ``!xs. ALL_DISTINCT xs ==> (LENGTH (REGISTER_LIST (reg_bitmap xs)) = LENGTH xs)``,
+  REPEAT STRIP_TAC \\ MATCH_MP_TAC ALL_DISTINCT_IMP_LENGTH_EQ
+  \\ ASM_SIMP_TAC std_ss [MEM_REGISTER_LIST_reg_bitmap]
+  \\ MATCH_MP_TAC SORTED_LO_IMP_ALL_DISTINCT \\ REWRITE_TAC [SORTED_REGISTER_LIST]);
+
+val ADDR_MODE4_UP_THM = prove(
+  ``!am4. (ADDR_MODE4_CMD am4).Up = ADDR_MODE4_UP am4``,
+  Cases_on `am4` \\ SRW_TAC [] [ADDR_MODE4_CMD_def,ADDR_MODE4_UP_def]);
+
+val WB_ADDRESS_EQ_ADDR_MODE4_WB' = prove(
+  ``!am4 x xs. ALL_DISTINCT xs ==> 
+         (WB_ADDRESS (ADDR_MODE4_CMD am4).Up (addr32 x) 
+             (LENGTH (REGISTER_LIST (reg_bitmap xs))) = 
+          addr32 (ADDR_MODE4_WB' am4 x (LENGTH xs)))``,
+  REWRITE_TAC [ADDR_MODE4_def,ADDR_MODE4_WB'_def,WB_ADDRESS_def,UP_DOWN_def]
+  \\ SIMP_TAC bool_ss [REGISTER_LIST_LENGTH,ADDR_MODE4_UP_THM] 
+  \\ REPEAT STRIP_TAC \\ Cases_on `ADDR_MODE4_UP am4` 
+  \\ ASM_REWRITE_TAC [addr32_ADD,addr32_SUB,addr32_n2w]);
+
+val ADDR_MODE4_ADDR'_def = Define `
+  (ADDR_MODE4_ADDR' (am4_DA wb) x y = y + 1w) /\ 
+  (ADDR_MODE4_ADDR' (am4_FA wb) x y = y + 1w) /\ 
+  (ADDR_MODE4_ADDR' (am4_IA wb) x y = x:word30) /\
+  (ADDR_MODE4_ADDR' (am4_FD wb) x y = x) /\
+  (ADDR_MODE4_ADDR' (am4_DB wb) x y = y) /\
+  (ADDR_MODE4_ADDR' (am4_EA wb) x y = y) /\
+  (ADDR_MODE4_ADDR' (am4_IB wb) x y = x + 1w) /\
+  (ADDR_MODE4_ADDR' (am4_ED wb) x y = x + 1w)`;
+
+val ADDR_MODE4_ADDR'_THM = prove(
+  ``!am4 x xs.
+      ALL_DISTINCT xs ==>
+      (FIRST_ADDRESS (ADDR_MODE4_CMD am4).Pre (ADDR_MODE4_CMD am4).Up
+        (addr32 x) (addr32 (ADDR_MODE4_WB' am4 x (LENGTH xs))) =
+       addr32 (ADDR_MODE4_ADDR' am4 x (ADDR_MODE4_WB' am4 x (LENGTH xs))))``,
+  Cases \\ SRW_TAC [] [ADDR_MODE4_ADDR'_def,FIRST_ADDRESS_def,ADDR_MODE4_CMD_def,addr32_SUC]);
+
+val ADDR_MODE4_ADDR_def = Define `
+  ADDR_MODE4_ADDR am4 x xs = ADDR_MODE4_ADDR' am4 x (ADDR_MODE4_WB' am4 x (LENGTH xs))`;
+
+val ADDRESS_LIST'_def = Define `
+  (ADDRESS_LIST' start 0 = []) /\
+  (ADDRESS_LIST' start (SUC n) = start :: ADDRESS_LIST' (start + 4w) n)`;
+
+val GENLIST_EQ = prove(
+  ``!xs f n. (!k. k < n ==> (f k = EL k xs)) /\ (n = LENGTH xs) ==> (GENLIST f n = xs)``,
+  recInduct SNOC_INDUCT \\ REPEAT STRIP_TAC 
+  \\ FULL_SIMP_TAC std_ss [LENGTH,GENLIST,LENGTH_SNOC,SNOC_11]
+  \\ `!k n. k < n ==> k < SUC n` by DECIDE_TAC
+  \\ `!k. k < LENGTH l ==> (f k = EL k l)` by METIS_TAC [EL_SNOC]
+  \\ `LENGTH l < SUC (LENGTH l)` by DECIDE_TAC
+  \\ `f (LENGTH l) = EL (LENGTH l) (SNOC x l)` by METIS_TAC []     
+  \\ ASM_REWRITE_TAC [EL_LENGTH_SNOC] 
+  \\ Q.PAT_ASSUM `!f. b ==> (GENLIST f g = l)` MATCH_MP_TAC
+  \\ ASM_REWRITE_TAC []);
+
+val ADDRESS_LIST'_INTRO = prove(
+  ``!n y. ADDRESS_LIST y n = ADDRESS_LIST' y n``,
+  REPEAT STRIP_TAC \\ REWRITE_TAC [ADDRESS_LIST_def] 
+  \\ MATCH_MP_TAC GENLIST_EQ \\ SIMP_TAC std_ss []
+  \\ Q.SPEC_TAC (`y`,`y`)
+  \\ Induct_on `n` THEN1 SRW_TAC [] [LENGTH,ADDRESS_LIST'_def]
+  \\ REPEAT STRIP_TAC << [
+    Cases_on `k` \\ REWRITE_TAC [EL,WORD_MULT_CLAUSES,
+       WORD_ADD_0,TL,HD,ADDRESS_LIST'_def,ADD1,GSYM word_add_n2w,WORD_ADD_ASSOC]
+    \\ FULL_SIMP_TAC std_ss [],
+    REWRITE_TAC [ADDRESS_LIST'_def,LENGTH] \\ METIS_TAC []]);
+
+val ADDR_MODE4_ADDRESSES_def = Define `
+  ADDR_MODE4_ADDRESSES am4 x xs = 
+    ADDRESS_LIST' (addr32 (ADDR_MODE4_ADDR am4 x xs)) (LENGTH xs)`;
+
+val ADDR_MODE4_FORMAT = prove(
+  ``!am4 x xs.
+      ALL_DISTINCT xs ==> 
+      (ADDR_MODE4 (ADDR_MODE4_CMD am4).Pre 
+          (ADDR_MODE4_CMD am4).Up (addr32 x) 
+          (reg_bitmap xs) =
+       (LEAST_SORT xs,
+        ADDR_MODE4_ADDRESSES am4 x xs,
+        addr32 (ADDR_MODE4_WB' am4 x (LENGTH xs))))``,
+  SIMP_TAC std_ss [LET_DEF,ADDR_MODE4_def,WB_ADDRESS_EQ_ADDR_MODE4_WB',REGISTER_LIST_LENGTH]
+  \\ SIMP_TAC std_ss [REGISTER_LIST_EQ_LEAST_SORT,ADDR_MODE4_ADDRESSES_def,
+                      ADDR_MODE4_ADDR'_THM,ADDR_MODE4_ADDR_def,ADDRESS_LIST'_INTRO]);
+
+val ADDR_MODE4_WB_THM = prove(
+  ``!am4 p xs. 
+      (reg Rd s = addr32 p) ==>
+      ((if (ADDR_MODE4_CMD am4).Wb then
+         INC_PC (REG_WRITE s.registers (state_mode s) Rd
+           (addr32 (ADDR_MODE4_WB' am4 p (LENGTH (MAP FST xs)))))
+        else INC_PC s.registers) =
+       INC_PC (REG_WRITE s.registers (state_mode s) Rd
+         (addr32 (ADDR_MODE4_WB am4 p (MAP FST xs)))))``,
+  REPEAT STRIP_TAC 
+  \\ `!am4. (ADDR_MODE4_CMD am4).Wb = ADDR_MODE4_wb am4` by 
+        (Cases \\ SRW_TAC [] [ADDR_MODE4_CMD_def,ADDR_MODE4_wb_def])
+  \\ ASM_REWRITE_TAC [ADDR_MODE4_WB_def] 
+  \\ Cases_on `ADDR_MODE4_wb am4` \\ ASM_REWRITE_TAC []
+  \\ Q.PAT_ASSUM `reg Rd s = addr32 p` (ASSUME_TAC o SYM)
+  \\ ASM_REWRITE_TAC [reg_def]
+  \\ Cases_on `Rd = 15w` \\ ASM_SIMP_TAC std_ss [REG_WRITE_READ]
+  \\ ASM_SIMP_TAC (std_ss++wordsLib.SIZES_ss) 
+       [REG_WRITE_def,mode_reg2num_def,num2register_thm,LET_DEF,
+        EVAL ``w2n (15w:word4)``,INC_PC_def,SUBST_def]);
+
+(* LDM instruction ------------------------------------------------------------- *)
+
+val LDM_VALUES_def = Define `
+  LDM_VALUES am4 x xs s = 
+    ZIP (LEAST_SORT xs, MAP (s.memory o ADDR30) (ADDR_MODE4_ADDRESSES am4 x xs))`;
+
+val MEM_MAP_FST_ZIP = prove(
+  ``!xs ys x. (LENGTH xs = LENGTH ys) ==> (MEM x (MAP FST (ZIP (xs,ys))) = MEM x xs)``,
+  Induct \\ Cases_on `ys` \\ SIMP_TAC std_ss [LENGTH,ZIP,MAP,MEM]
+  THEN1 REWRITE_TAC [SUC_NOT] THEN1 METIS_TAC [SUC_NOT] \\ ASM_SIMP_TAC std_ss [MEM]);
+
+val ALL_DISTINCT_MAP_FST_ZIP = prove(
+  ``!xs ys. (LENGTH xs = LENGTH ys) ==> 
+            (ALL_DISTINCT (MAP FST (ZIP (xs,ys))) = ALL_DISTINCT xs)``,
+  Induct \\ Cases_on `ys` \\ SIMP_TAC std_ss [LENGTH]
+  THEN1 SRW_TAC [] [ZIP,MAP,FST,ALL_DISTINCT]
+  THEN1 REWRITE_TAC [SUC_NOT] THEN1 METIS_TAC [SUC_NOT]
+  \\ ASM_SIMP_TAC bool_ss [ZIP,MAP,FST,ALL_DISTINCT,MEM_MAP_FST_ZIP]);  
+
+val SORTED_LOWER_IMP_ALL_DISTINCT = prove(
+  ``!xs. SORTED $<+ xs ==> ALL_DISTINCT xs``,
+  Induct \\ SIMP_TAC std_ss [ALL_DISTINCT] \\ REPEAT STRIP_TAC
+  \\ IMP_RES_TAC SORTED_EQ_LOWER \\ METIS_TAC [WORD_LOWER_REFL]);
+
+val ALL_DISTINCT_LEAST_SORT = prove(
+  ``!xs. ALL_DISTINCT (LEAST_SORT xs)``,
+  STRIP_TAC \\ MATCH_MP_TAC SORTED_LOWER_IMP_ALL_DISTINCT
+  \\ REWRITE_TAC [SORTED_LEAST_SORT]);
+
+val REG_WRITEL_INTRO = prove(
+  ``!l r m. 
+      ALL_DISTINCT (MAP FST l) ==>
+      (FOLDL (\reg' (rp,rd). REG_WRITE reg' m rp rd) r l = REG_WRITEL r m l)``,
+  Induct \\ SIMP_TAC std_ss [FOLDL,REG_WRITEL_def] \\ REPEAT STRIP_TAC
+  \\ Cases_on `h` \\ FULL_SIMP_TAC std_ss [REG_WRITEL_def,ALL_DISTINCT,MAP,FST]
+  \\ `!l. ~MEM q (MAP FST l) ==> 
+    (REG_WRITEL (REG_WRITE r m q r') m l = REG_WRITE (REG_WRITEL r m l) m q r')` 
+          by ALL_TAC << [
+    Induct \\ SIMP_TAC bool_ss [REG_WRITEL_def,MEM,MAP,FST] \\ REPEAT STRIP_TAC
+    \\ Cases_on `h` \\ FULL_SIMP_TAC std_ss [REG_WRITEL_def] 
+    \\ MATCH_MP_TAC REG_WRITE_WRITE_COMM \\ ASM_REWRITE_TAC [],
+  METIS_TAC []]);
+
+val LENGTH_ADDRESS_LIST' = prove(
+  ``!n x. LENGTH (ADDRESS_LIST' x n) = n``,
+  Induct \\ SRW_TAC [] [LENGTH,ADDRESS_LIST'_def]);
+
+val LDM_WRITEL_INTRO_LEMMA = prove(
+  ``!xs. 
+      ALL_DISTINCT xs ==> 
+      (LENGTH (LEAST_SORT xs) = 
+       LENGTH (MAP g (ADDR_MODE4_ADDRESSES am4 x xs)))``,
+  SIMP_TAC std_ss 
+    [LENGTH_LEAST_SORT,ADDR_MODE4_ADDRESSES_def,LENGTH_ADDRESS_LIST',LENGTH_MAP]);
+  
+val LDM_WRITEL_INTRO = prove(
+  ``!xs r m. 
+      ALL_DISTINCT xs ==>
+      (FOLDL (\reg' (rp,rd). REG_WRITE reg' m rp rd) r (LDM_VALUES am4 x xs s) = 
+       REG_WRITEL r m (LDM_VALUES am4 x xs s))``,
+  REPEAT STRIP_TAC \\ MATCH_MP_TAC REG_WRITEL_INTRO
+  \\ `LENGTH (LEAST_SORT xs) = 
+      LENGTH (MAP (s.memory o ADDR30) (ADDR_MODE4_ADDRESSES am4 x xs))`
+             by ASM_SIMP_TAC std_ss [LENGTH_LEAST_SORT,LENGTH_ADDRESS_LIST',
+                                     ADDR_MODE4_ADDRESSES_def,LENGTH_MAP]
+  \\ IMP_RES_TAC ALL_DISTINCT_MAP_FST_ZIP
+  \\ ASM_SIMP_TAC std_ss [LDM_VALUES_def,ALL_DISTINCT_LEAST_SORT]);
+
+val LDM_STATE_def = Define `
+  LDM_STATE am4 p xs Rd s =
+  <|registers :=
+            REG_WRITEL
+              (INC_PC
+                 (REG_WRITE s.registers (state_mode s) Rd
+                    (addr32 (ADDR_MODE4_WB am4 p (MAP FST xs)))))
+              (state_mode s)
+              (ZIP
+                 (LEAST_SORT (MAP FST xs),
+                  MAP (s.memory o ADDR30)
+                    (ADDRESS_LIST'
+                       (addr32 (ADDR_MODE4_ADDR am4 p (MAP FST xs)))
+                       (LENGTH (MAP FST xs))))); psrs := s.psrs;
+          memory := s.memory; undefined := F|>`;
+
+val ldm = simple_clean ARM_LDM [``~(Rd = 15w:word4)``]
+val ldm = Q.INST [`opt`|->`ADDR_MODE4_CMD am4`] ldm
+val ldm = Q.INST [`list`|->`reg_bitmap (MAP FST (xs:(word4 # word32) list))`] ldm
+val ldm = REWRITE_RULE [NOT_ADDR_MODE4_BSN] ldm
+val ldm = DISCH ``reg Rd s = addr32 p`` ldm
+val ldm = DISCH ``ALL_DISTINCT (MAP FST (xs:(word4 # word32) list))`` ldm
+val ldm = SIMP_RULE bool_ss [ADDR_MODE4_FORMAT,FST,SND,ADDR_MODE4_WB_THM,
+                             GSYM LDM_VALUES_def,LDM_WRITEL_INTRO] ldm
+val ldm = REWRITE_RULE [LDM_VALUES_def,GSYM LDM_STATE_def,ADDR_MODE4_ADDRESSES_def] ldm
+
+
+val reg_values_def = Define ` 
+  reg_values = MAP SND o QSORT (\x y. FST x <=+ FST y)`;
+  
+val LDM_PRE_EXPANSION = let
+  val xs = `(15w,SOME x1)::(a,SOME x2)::xs`;
+  val ys = `[(b1,xM_seq [y1]);(b3,xM_seq y3)]`;
+  val (st,ud,rt,cd) = (`(T,st)`,`(T,ud)`,`(F,rt)`,`(T,g)`);
+  val th = sep_pred_semantics (xs,ys,st,ud,rt,cd);
+  in th end;
+
+val LDM_POST_EXPANSION = let
+  val xs = `(15w,SOME x1)::(a,SOME x2)::xs`;
+  val ys = `[(b1,xM_seq [y1]);(b3,xM_seq y3)]`;
+  val (st,ud,rt,cd) = (`(T,st)`,`(T,ud)`,`(F,rt)`,`(F,g)`);
+  val th = sep_pred_semantics (xs,ys,st,ud,rt,cd);
+  in th end;
+
+val LDM_SIMP_LEMMA = prove(
+  ``!xs. (MAP FST (MAP (\x. (FST x,NONE)) xs) = MAP FST xs) /\ 
+         (MAP FST (MAP (\x. (FST x,SOME (SND x))) xs) = MAP FST xs)``,
+  Induct \\ SRW_TAC [] []);
+
+val MEM_LOWEST = prove(
+  ``!xs. 0 < LENGTH xs ==> ?h. MEM h xs /\ !x. MEM x xs ==> h <=+ x``,
+  Induct \\ FULL_SIMP_TAC std_ss [LENGTH,MEM] \\ REPEAT STRIP_TAC  
+  \\ Cases_on `?y. MEM y xs /\ y <=+ h` << [  
+    `?y. MEM y xs /\ y <=+ h` by METIS_TAC []
+    \\ Cases_on `xs` THEN1 FULL_SIMP_TAC std_ss [MEM]
+    \\ FULL_SIMP_TAC bool_ss [LENGTH,DECIDE ``0 < SUC n = T``]
+    \\ Q.EXISTS_TAC `h''` \\ ASM_REWRITE_TAC []
+    \\ METIS_TAC [WORD_LOWER_EQ_TRANS],
+    Q.EXISTS_TAC `h` \\ FULL_SIMP_TAC bool_ss []
+    \\ METIS_TAC [WORD_LOWER_EQ_CASES,WORD_LOWER_EQ_REFL]]);
+
+val PERM_IMPs = prove(
+  ``!xs ys. PERM xs ys ==> (LENGTH xs = LENGTH ys) /\ !x. MEM x xs = MEM x ys``,
+  Induct \\ SIMP_TAC bool_ss [PERM_NIL,PERM_CONS_EQ_APPEND,LENGTH]
+  \\ REPEAT STRIP_TAC \\ ASM_REWRITE_TAC []
+  \\ Q.PAT_ASSUM `!ys. b:bool` IMP_RES_TAC 
+  \\ FULL_SIMP_TAC std_ss [LENGTH_APPEND,LENGTH,MEM,MEM_APPEND] THEN1 DECIDE_TAC
+  \\ EQ_TAC \\ REPEAT STRIP_TAC \\ ASM_SIMP_TAC bool_ss []);
+
+val LDM_mem_SIMP = prove(
+  ``!ys y s g. 
+      ms_sem y ys <|registers := g; psrs := s.psrs; memory := s.memory; undefined := F|> =
+      ms_sem y ys s``,
+  Induct \\ SRW_TAC [] [ms_sem_def,mem_def]);
+
+val LDM_VALUES_0 = prove(
+  ``!xs.
+      (0 = LENGTH xs) ==> 
+      (ZIP (LEAST_SORT xs,
+            MAP (s.memory o ADDR30) (ADDRESS_LIST' (addr32 y) (LENGTH xs))) = [])``,
+  Cases \\ SRW_TAC [] [LENGTH,LEAST_SORT_def,ADDR_MODE4_ADDRESSES_def,ADDRESS_LIST'_def]);
+
+val LDM_VALUES_SUC = prove(
+  ``!xs:word4 list n. 
+      ALL_DISTINCT xs ==> (SUC n = LENGTH xs) ==> 
+      ?ys. 
+        !y. (ZIP
+              (LEAST_SORT xs,
+                MAP (s.memory o ADDR30) (ADDRESS_LIST' (addr32 y) (LENGTH xs))) = 
+              (LEAST_MEM xs,s.memory y)::
+                ZIP
+                  (LEAST_SORT ys,
+                 MAP (s.memory o ADDR30) (ADDRESS_LIST' (addr32 (y+1w)) (LENGTH ys)))) /\
+           (n = LENGTH ys) /\ ALL_DISTINCT ys /\ !x. MEM x (LEAST_MEM xs::ys) = MEM x xs``,
+  REPEAT STRIP_TAC \\ Cases_on `xs` 
+  \\ FULL_SIMP_TAC std_ss [LENGTH] THEN1 METIS_TAC [SUC_NOT]
+  \\ FULL_SIMP_TAC std_ss [LEAST_SORT_def,LET_DEF,ADDRESS_LIST'_def,MAP,ADDR30_def,
+     GSYM addr30_def,addr30_addr32,ZIP,CONS_11]  
+  \\ Q.EXISTS_TAC `FILTER (\x. ~(x = LEAST_MEM (h::t))) (h::t)`  
+  \\ `MEM (LEAST_MEM (h::t)) (h::t)` by METIS_TAC [MEM_LEAST_MEM]
+  \\ IMP_RES_TAC LENGTH_FILTER_NEQ  
+  \\ FULL_SIMP_TAC bool_ss [LENGTH,ADD1,ADD_SUB,addr32_SUC]
+  \\ REPEAT STRIP_TAC THEN1 METIS_TAC [ALL_DISTINCT_FILTER]  
+  \\ SIMP_TAC std_ss [MEM,MEM_FILTER]
+  \\ Cases_on `x = LEAST_MEM (h::t)` \\ ASM_REWRITE_TAC []
+  \\ METIS_TAC [MEM_LEAST_MEM,MEM]);
+  
+val MEM_NOT_MEM_IMP_NEQ = prove(
+  ``!xs x y. MEM x xs /\ ~MEM y xs ==> ~(x = y)``,
+  REPEAT STRIP_TAC
+  \\ `?ys zs. xs = ys ++ [x] ++ zs` by METIS_TAC [MEM_EQ_EXISTS]
+  \\ FULL_SIMP_TAC std_ss [MEM_APPEND,MEM]);
+
+val reg_15_LDM_STATE = prove(
+  ``ALL_DISTINCT (MAP FST xs) /\ (reg 15w s = addr32 p) /\ 
+    ~MEM 15w (MAP FST xs) /\ ~(a = 15w) ==>
+    (reg 15w (LDM_STATE am4 x xs a s) = addr32 (pcADD 1w p))``,
+  SIMP_TAC (srw_ss()) [LDM_STATE_def,reg_def] 
+  \\ Q.SPEC_TAC (`addr32 (ADDR_MODE4_WB am4 x (MAP FST xs))`,`y`)
+  \\ `LENGTH xs = LENGTH (MAP FST xs)` by METIS_TAC [LENGTH_MAP]
+  \\ ASM_REWRITE_TAC [] \\ POP_ASSUM (fn th => ALL_TAC)
+  \\ Q.SPEC_TAC (`MAP FST xs`,`xs`) \\ STRIP_TAC
+  \\ Q.SPEC_TAC (`ADDR_MODE4_ADDR am4 x xs`,`w`)
+  \\ Induct_on `LENGTH xs` << [
+    SIMP_TAC std_ss [LDM_VALUES_0,REG_WRITEL_def,INC_PC_r15,REG_WRITE_r15,pcADD_def] 
+    \\ ONCE_REWRITE_TAC [WORD_ADD_COMM] \\ REWRITE_TAC [addr32_SUC] 
+    \\ METIS_TAC [WORD_ADD_COMM],  
+    REPEAT STRIP_TAC
+    \\ (STRIP_ASSUME_TAC o UNDISCH_ALL o Q.SPECL [`xs`,`v`]) LDM_VALUES_SUC
+    \\ FULL_SIMP_TAC bool_ss [REG_WRITEL_def]    
+    \\ Cases_on `xs` THEN1 METIS_TAC [LENGTH,SUC_NOT]
+    \\ `MEM (LEAST_MEM (h::t)) (h::t)` by METIS_TAC [MEM_LEAST_MEM]    
+    \\ IMP_RES_TAC MEM_NOT_MEM_IMP_NEQ
+    \\ ASM_SIMP_TAC std_ss [REG_WRITE_r15]
+    \\ `~MEM 15w ys` by METIS_TAC [MEM]
+    \\ `ALL_DISTINCT ys` by METIS_TAC []
+    \\ `LENGTH ys = LENGTH ys` by REWRITE_TAC []
+    \\ Q.PAT_ASSUM `!xs'. b ==> c:bool` 
+           (STRIP_ASSUME_TAC o UD_ALL o Q.SPECL [`w+1w`,`y`] o UD_ALL o Q.SPEC `ys`)]);
+
+val state_mode_simp = prove(
+  ``state_mode <|registers := r; psrs := s.psrs; memory := m; undefined := b|> =
+    state_mode s``,SRW_TAC [] [state_mode_def]);
+
+val reg_wb_LDM_STATE = prove(
+  ``ALL_DISTINCT (MAP FST xs) /\ ~MEM a (MAP FST xs) /\ ~(a = 15w) ==>
+    (reg a (LDM_STATE am4 x xs a s) = addr32 (ADDR_MODE4_WB am4 x xs))``,
+  SIMP_TAC (srw_ss()) [LDM_STATE_def,reg_def,ADDR_MODE4_WB_def] 
+  \\ `LENGTH xs = LENGTH (MAP FST xs)` by METIS_TAC [LENGTH_MAP]
+  \\ ASM_REWRITE_TAC [] \\ POP_ASSUM (fn th => ALL_TAC)
+  \\ REWRITE_TAC [GSYM ADDR_MODE4_WB_def] 
+  \\ Q.SPEC_TAC (`addr32 (ADDR_MODE4_WB am4 x (MAP FST xs))`,`y`)
+  \\ Q.SPEC_TAC (`ADDR_MODE4_ADDR am4 x (MAP FST xs)`,`w`)
+  \\ Q.SPEC_TAC (`MAP FST xs`,`xs`) \\ STRIP_TAC
+  \\ REWRITE_TAC [state_mode_simp]
+  \\ Induct_on `LENGTH xs`
+  THEN1 SIMP_TAC std_ss [LDM_VALUES_0,REG_WRITEL_def,REG_READ_INC_PC,
+    REG_READ_WRITE_NEQ,pcADD_def,REG_READ_WRITE] 
+  \\ REPEAT STRIP_TAC
+  \\ (STRIP_ASSUME_TAC o UNDISCH_ALL o Q.SPECL [`xs`,`v`]) LDM_VALUES_SUC
+  \\ FULL_SIMP_TAC bool_ss [REG_WRITEL_def]    
+  \\ Cases_on `xs` THEN1 METIS_TAC [LENGTH,SUC_NOT]
+  \\ `MEM (LEAST_MEM (h::t)) (h::t)` by METIS_TAC [MEM_LEAST_MEM]    
+  \\ IMP_RES_TAC MEM_NOT_MEM_IMP_NEQ
+  \\ ASM_SIMP_TAC std_ss [REG_READ_WRITE_NEQ2]
+  \\ `~MEM a ys` by METIS_TAC [MEM]
+  \\ `ALL_DISTINCT ys` by METIS_TAC []
+  \\ `LENGTH ys = LENGTH ys` by REWRITE_TAC []
+  \\ Q.PAT_ASSUM `!xs'. b ==> c:bool` 
+           (STRIP_ASSUME_TAC o UD_ALL o Q.SPECL [`w+1w`,`y`] o UD_ALL o Q.SPEC `ys`));
+
+val xR_list_sem_PERM_LEMMA = prove(
+  ``!xs ys h. xR_list_sem (xs++h::ys) = xR_list_sem (h::(xs++ys))``,
+  Induct \\ SIMP_TAC std_ss [xR_list_def,FUN_EQ_THM,APPEND]
+  \\ Cases_on `h` \\ Cases_on `r` \\ ASM_REWRITE_TAC [xR_list_sem_def]
+  \\ Cases_on `h'` \\ Cases_on `r` \\ ASM_REWRITE_TAC [xR_list_sem_def]
+  \\ REPEAT STRIP_TAC \\ EQ_TAC \\ SIMP_TAC std_ss []);
+
+val xR_list_sem_PERM = prove(
+  ``!xs ys. PERM xs ys ==> (xR_list_sem xs = xR_list_sem ys)``,
+  REWRITE_TAC [FUN_EQ_THM] 
+  \\ Induct \\ SIMP_TAC bool_ss [PERM_NIL,PERM_CONS_EQ_APPEND] \\ REPEAT STRIP_TAC
+  \\ ASM_REWRITE_TAC [xR_list_sem_PERM_LEMMA]
+  \\ Cases_on `h` \\ Cases_on `r` \\ ASM_REWRITE_TAC [xR_list_sem_def]
+  \\ METIS_TAC []);
+
+val PERM_MAP = prove(
+  ``!xs ys. PERM xs ys ==> PERM (MAP f xs) (MAP f ys)``,
+  Induct \\ SIMP_TAC bool_ss [PERM_NIL,PERM_CONS_EQ_APPEND,PERM_REFL] \\ REPEAT STRIP_TAC
+  \\ ASM_REWRITE_TAC [MAP,MAP_APPEND] \\ ONCE_REWRITE_TAC [PERM_SYM]
+  \\ MATCH_MP_TAC APPEND_PERM_SYM \\ REWRITE_TAC [APPEND,PERM_CONS_IFF]
+  \\ MATCH_MP_TAC APPEND_PERM_SYM \\ ONCE_REWRITE_TAC [PERM_SYM]
+  \\ ASM_SIMP_TAC bool_ss [GSYM MAP_APPEND]);
+
+val SORTS_QSORT_FST_LOWER_EQ = prove(
+  ``SORTS QSORT (\x y. FST x <=+ FST y)``,
+  MATCH_MP_TAC QSORT_SORTS \\ REWRITE_TAC [transitive_def,total_def] 
+  \\ REPEAT STRIP_TAC \\ Cases_on `x` \\ Cases_on `y`
+  \\ FULL_SIMP_TAC std_ss [WORD_LOWER_EQ_CASES]
+  \\ Cases_on `z` \\ FULL_SIMP_TAC std_ss [] \\ MATCH_MP_TAC WORD_LOWER_EQ_TRANS 
+  \\ Q.EXISTS_TAC `q'` \\ ASM_REWRITE_TAC []);
+
+val LENGTH_reg_values = prove(
+  ``!xs. LENGTH (reg_values xs) = LENGTH xs``,
+  SIMP_TAC std_ss [reg_values_def,LENGTH_MAP] \\ REPEAT STRIP_TAC 
+  \\ MATCH_MP_TAC PERM_LENGTH \\ METIS_TAC [SORTS_QSORT_FST_LOWER_EQ,SORTS_DEF,PERM_SYM]);
+
+val xR_list_sem_QSORT_INTRO = prove(
+  ``!f xs. 
+       xR_list_sem (MAP f xs) = xR_list_sem ((MAP f o QSORT (\x y. FST x <=+ FST y)) xs)``,
+  REPEAT STRIP_TAC \\ MATCH_MP_TAC xR_list_sem_PERM \\ SIMP_TAC std_ss []
+  \\ MATCH_MP_TAC PERM_MAP \\ METIS_TAC [SORTS_QSORT_FST_LOWER_EQ,SORTS_DEF]);
+
+val MEM_ALL_MEM_ALL_MAP = prove(
+  ``!xs ys. (!a. MEM a xs = MEM a ys) ==> (!a. MEM a (MAP f xs) = MEM a (MAP f ys))``,
+  REPEAT STRIP_TAC \\ REWRITE_TAC [MEM_MAP] \\ EQ_TAC \\ REPEAT STRIP_TAC
+  \\ Q.EXISTS_TAC `y` \\ ASM_REWRITE_TAC [] \\ METIS_TAC []);
+
+val MEM_MAP_QSORT_INTRO = prove(
+  ``!xs a. MEM a (MAP FST xs) = MEM a ((MAP FST o QSORT (\x y. FST x <=+ FST y)) xs)``,
+  SIMP_TAC std_ss [] \\ STRIP_TAC \\ MATCH_MP_TAC MEM_ALL_MEM_ALL_MAP
+  \\ MATCH_MP_TAC PERM_IMP_MEM_EQUALITY \\ METIS_TAC [SORTS_QSORT_FST_LOWER_EQ,SORTS_DEF]);
+
+val PERM_IMP_ALL_DISTINCT_EQ = prove(
+  ``!xs ys. PERM xs ys ==> (ALL_DISTINCT xs = ALL_DISTINCT ys)``,
+  Induct \\ SIMP_TAC bool_ss [PERM_NIL,PERM_CONS_EQ_APPEND] \\ REPEAT STRIP_TAC
+  \\ ASM_REWRITE_TAC [ALL_DISTINCT] \\ IMP_RES_TAC PERM_IMP_MEM_EQUALITY
+  \\ `!M'. ALL_DISTINCT (M' ++ h::N) = ALL_DISTINCT (h::(M' ++ N))` by     
+        (Induct \\ ASM_SIMP_TAC bool_ss [APPEND,ALL_DISTINCT,MEM,MEM_APPEND]
+         \\ REPEAT STRIP_TAC \\ EQ_TAC \\ SIMP_TAC std_ss [])
+  \\ ASM_SIMP_TAC bool_ss [ALL_DISTINCT] \\ METIS_TAC []);
+
+val ALL_DISTINCT_QSORT_INTRO = prove(
+  ``!xs. ALL_DISTINCT (MAP FST xs) =
+         ALL_DISTINCT ((MAP FST o QSORT (\x y. FST x <=+ FST y)) xs)``,
+  STRIP_TAC \\ MATCH_MP_TAC PERM_IMP_ALL_DISTINCT_EQ \\ SIMP_TAC std_ss []
+  \\ MATCH_MP_TAC PERM_MAP \\ METIS_TAC [SORTS_QSORT_FST_LOWER_EQ,SORTS_DEF]);
+
+val LENGTH_QSORT_INTRO = prove(
+  ``!xs. LENGTH (MAP FST xs) = LENGTH (QSORT (\x y. FST x <=+ FST y) xs)``,
+  STRIP_TAC \\ REWRITE_TAC [LENGTH_MAP] \\ MATCH_MP_TAC PERM_LENGTH 
+  \\ METIS_TAC [SORTS_QSORT_FST_LOWER_EQ,SORTS_DEF]);
+
+val SORTED_MAP = prove(
+  ``!xs f g. SORTED g (MAP f xs) = SORTED (\x y. g (f x) (f y)) xs``,
+  Induct \\ REWRITE_TAC [SORTED_DEF,MAP]
+  \\ Cases_on `xs` \\ FULL_SIMP_TAC std_ss [SORTED_DEF,MAP]);
+
+val LEAST_SORT_EQ_QSORT = prove(
+  ``!xs. ALL_DISTINCT (MAP FST xs) ==>
+         (LEAST_SORT (MAP FST xs) = MAP FST (QSORT (\x y. FST x <=+ FST y) xs))``,
+  REPEAT STRIP_TAC \\ MATCH_MP_TAC SORTED_LO_IMP_EQ  
+  \\ REWRITE_TAC [SORTED_LEAST_SORT,MEM_LEAST_SORT] \\ REPEAT STRIP_TAC << [
+    MATCH_MP_TAC SORTED_LO
+    \\ ASM_REWRITE_TAC [SIMP_RULE std_ss [] (GSYM ALL_DISTINCT_QSORT_INTRO)]
+    \\ REWRITE_TAC [SORTED_MAP] \\ METIS_TAC [SORTS_QSORT_FST_LOWER_EQ,SORTS_DEF],
+    SIMP_TAC std_ss [SIMP_RULE std_ss [] (GSYM MEM_MAP_QSORT_INTRO)]]);
+
+val xR_list_sem_IGNORE_REG_WRITE = prove(
+  ``!xs r q ax regs.
+      ~MEM q (MAP FST xs) ==>
+      (xR_list_sem (MAP (\x. (FST x,SOME (SND x))) xs)
+         <| registers := REG_WRITE regs (state_mode s) q r; 
+            psrs := s.psrs; memory := mt; undefined := bt |> =
+       xR_list_sem (MAP (\x. (FST x,SOME (SND x))) xs)
+         <| registers := regs; psrs := s.psrs; memory := mt; undefined := bt |>)``,
+  Induct THEN1 REWRITE_TAC [xR_list_sem_def,MAP] \\ Cases
+  \\ SIMP_TAC std_ss [MAP,xR_list_sem_def,MEM] \\ Cases_on `q = 15w`
+  \\ REPEAT STRIP_TAC \\ Q.PAT_ASSUM `!s.b` IMP_RES_TAC
+  \\ ASM_SIMP_TAC (srw_ss()) [reg_def,state_mode_simp,REG_READ_WRITE_NEQ2]
+  \\ `~(15w = q')` by METIS_TAC [] \\ ASM_SIMP_TAC std_ss [REG_WRITE_r15]);
+
+val xR_list_sem_LDM_STATE = prove(
+  ``ALL_DISTINCT (MAP FST xs) /\ 
+    ms_sem (ADDR_MODE4_ADDR am4 x xs) (reg_values xs) s ==>
+    xR_list_sem (MAP (\x. (FST x,SOME (SND x))) xs) (LDM_STATE am4 x xs a s)``,
+  REWRITE_TAC [LDM_STATE_def,ADDR_MODE4_ADDR_def,reg_values_def]     
+  \\ `LENGTH xs = LENGTH (MAP FST xs)` by METIS_TAC [LENGTH_MAP]
+  \\ ASM_REWRITE_TAC [] \\ POP_ASSUM (fn th => ALL_TAC)
+  \\ REWRITE_TAC [GSYM ADDR_MODE4_ADDR_def] 
+  \\ Q.SPEC_TAC (`ADDR_MODE4_ADDR am4 x (MAP FST xs)`,`ax`)
+  \\ Q.SPEC_TAC (`addr32 (ADDR_MODE4_WB am4 x (MAP FST xs))`,`y`)
+  \\ SIMP_TAC bool_ss [LEAST_SORT_EQ_QSORT]
+  \\ REWRITE_TAC [xR_list_sem_QSORT_INTRO,MEM_MAP_QSORT_INTRO,
+                  ALL_DISTINCT_QSORT_INTRO,LENGTH_QSORT_INTRO]
+  \\ SIMP_TAC std_ss [] \\ Q.SPEC_TAC (`QSORT (\x y. FST x <=+ FST y) xs`,`xs`)
+  \\ Induct \\ REWRITE_TAC [MAP,xR_list_sem_def]
+  \\ Cases \\ SIMP_TAC (srw_ss()) [xR_list_sem_def,reg_def,MEM,state_mode_simp,ms_sem_def]
+  \\ SIMP_TAC std_ss [ADDRESS_LIST'_def,MAP,ADDR30_def,GSYM addr30_def,addr30_addr32,ZIP]
+  \\ SIMP_TAC bool_ss [REG_WRITEL_def,REG_READ_WRITE,mem_def,REG_WRITE_15]
+  \\ ASM_SIMP_TAC bool_ss [xR_list_sem_IGNORE_REG_WRITE,GSYM addr32_SUC] \\ METIS_TAC []);
+
+val status_LDM_STATE = prove(
+  ``status (LDM_STATE am4 x xs a s) = status s``,
+  SRW_TAC [] [LDM_STATE_def,status_def,statusN_def,statusZ_def,statusC_def,statusV_def]);
+
+val mem_LDM_STATE = prove(
+  ``mem p (LDM_STATE am4 x xs a s) = mem p s``,
+  SRW_TAC [] [LDM_STATE_def,mem_def]);
+
+val ms_sem_LDM_STATE = prove(
+  ``ms_sem x xs (LDM_STATE am4 y ys a s) = ms_sem x xs s``,
+  Q.SPEC_TAC (`x`,`x`) \\ Induct_on `xs` \\ ASM_REWRITE_TAC [ms_sem_def,mem_LDM_STATE]);
+
+val undef_LDM_STATE = prove(
+  ``(LDM_STATE am4 x xs a s).undefined = F``, SRW_TAC [] [LDM_STATE_def]);
+
+val owrt_visible_LDM_STATE = prove(
+  ``owrt_visible (LDM_STATE am4 x xs a s) = owrt_visible s``,
+  SRW_TAC [] [owrt_visible_def,LDM_STATE_def,set_status_def,owrt_visible_regs_def,
+              state_mode_simp,REG_OWRT_ALL]);
+
+val xs = `[(a1,SOME x1)]`;
+val ys = `[(b1,xM_seq [y1])]`;
+val (st,ud,rt,cd) = (`(T,st)`,`(T,ud)`,`(F,rt)`,`(F,g)`);
+val NOP_sem = sep_pred_semantics (xs,ys,st,ud,rt,cd);
+
+val IMP_ARM_NOP = prove(
+  ``(!state cpsr.
+       (state.memory ((31 >< 2) (state.registers r15)) = cmd) /\
+       Abbrev (cpsr = CPSR_READ state.psrs) /\
+       ~CONDITION_PASSED2 (NZCV cpsr) c /\ ~state.undefined ==>
+       (NEXT_ARM_MEM state =
+        <|registers := INC_PC state.registers; psrs := state.psrs;
+          memory := state.memory; undefined := F|>)) ==>
+    ARM_NOP c [cmd]``,
+  REPEAT STRIP_TAC \\ REWRITE_TAC [ARM_NOP_def,ARM_PROG1_EQ,nPASS_def]  
+  \\ MOVE_STAR_TAC `st*cc*mp*pc*ud` `cc*(st*mp*pc*ud)`
+  \\ REWRITE_TAC [cond_STAR]
+  \\ MOVE_STAR_TAC `st*mp*pc*ud` `pc*mp*st*ud`
+  \\ SIMP_TAC bool_ss [NOP_sem,ALL_DISTINCT,MEM,ALL_DISJOINT_def,EVERY_DEF,mem_def,reg_def]
+  \\ FULL_SIMP_TAC bool_ss [markerTheory.Abbrev_def,GSYM addr30_def,GSYM status_THM]
+  \\ REPEAT STRIP_TAC \\ Q.EXISTS_TAC `1` \\ REWRITE_TAC [STATE_ARM_MEM_1]
+  \\ `s.memory (addr30 (s.registers r15)) = cmd` by METIS_TAC [addr30_addr32]
+  \\ Q.PAT_ASSUM `!state. b:bool` (STRIP_ASSUME_TAC o Q.SPEC `s`)
+  \\ FULL_SIMP_TAC (srw_ss()) [status_THM,INC_PC_r15,pcADD_def,GSYM addr32_SUC]
+  \\ STRIP_TAC THEN1 METIS_TAC [WORD_ADD_COMM] 
+  \\ REWRITE_TAC [arm2set''_EQ,IN_INSERT,NOT_IN_EMPTY]
+  \\ ASM_SIMP_TAC (srw_ss()) [reg_def,mem_def,REG_READ_INC_PC,state_mode_def,
+      owrt_visible_def,set_status_def,owrt_visible_regs_def,REG_OWRT_ALL]);  
+
+fun MAKE_ARM_NOP nop_rule = 
+  MATCH_MP IMP_ARM_NOP ((Q.GEN `state` o Q.GEN `cpsr` o SPEC_ALL) nop_rule);
+
+val IMP_ARM_PROG2 = prove(
+  ``ARM_NOP c cs ==> (ARM_PROG P cs {} Q Z ==> ARM_PROG2 c P cs Q Z)``,
+  SIMP_TAC std_ss [ARM_PROG2_def]);
+
+fun MAKE_PROG2 th nop_rule = 
+  MATCH_MP (MATCH_MP IMP_ARM_PROG2 (MAKE_ARM_NOP nop_rule)) th;
+
+val raw_LDM = prove(
+  ``ARM_PROG 
+     (R30 a x * 
+      xR_list (MAP (\x.(FST x,NONE)) xs) * 
+      ms (ADDR_MODE4_ADDR am4 x xs) (reg_values xs) * S st * PASS c st) 
+     [enc (LDM c (ADDR_MODE4_CMD am4) a (reg_bitmap (MAP FST xs)))] {}
+     (R30 a (ADDR_MODE4_WB am4 x xs) *
+      xR_list (MAP (\x.(FST x,SOME (SND x))) xs) *
+      ms (ADDR_MODE4_ADDR am4 x xs) (reg_values xs) * S st) {}``,
+  ARM_PROG_INIT_TAC 
+  \\ ASM_MOVE_STAR_TAC `a*xs*mm*st*cd*cmd*pc*ud` `pc*a*xs*cmd*mm*st*ud*cd`
+  \\ MOVE_STAR_TAC `a*xs*mm*st*cmd*pc*ud` `pc*a*xs*cmd*mm*st*ud`
+  \\ FULL_SIMP_TAC bool_ss [R30_def,LDM_PRE_EXPANSION,LDM_POST_EXPANSION,
+         LDM_SIMP_LEMMA,ALL_DISTINCT,MEM]
+  \\ `CONDITION_PASSED2 (status s) c` by METIS_TAC []
+  \\ `mem (addr30 (reg 15w s)) s =
+      enc (LDM c (ADDR_MODE4_CMD am4) a (reg_bitmap (MAP FST xs)))` 
+         by METIS_TAC [addr30_addr32]
+  \\ `~(a = 15w)` by METIS_TAC []
+  \\ ASSUME_TAC ((UNDISCH o UNDISCH o UNDISCH o UNDISCH o UNDISCH o UNDISCH o 
+                  Q.INST [`p`|->`x`,`Rd`|->`a`]) ldm)
+  \\ ASM_REWRITE_TAC [] \\ PAT_ASSUM `` NEXT_ARM_MEM s = s'`` (fn th => ALL_TAC)
+  \\ STRIP_TAC 
+  THEN1 ASM_SIMP_TAC bool_ss [reg_15_LDM_STATE,reg_wb_LDM_STATE,xR_list_sem_LDM_STATE,
+     status_LDM_STATE,mem_LDM_STATE,ms_sem_LDM_STATE,undef_LDM_STATE]
+  \\ REWRITE_TAC [arm2set''_EQ,mem_LDM_STATE,owrt_visible_LDM_STATE]
+  \\ SIMP_TAC (srw_ss()) [IN_INSERT,IN_LIST_TO_SET,LDM_STATE_def,reg_def,state_mode_simp]
+  \\ `LENGTH xs = LENGTH (MAP FST xs)` by METIS_TAC [LENGTH_MAP]
+  \\ ASM_SIMP_TAC bool_ss [LEAST_SORT_EQ_QSORT]
+  \\ Q.SPEC_TAC (`ADDR_MODE4_ADDR am4 x (MAP FST xs)`,`ax`)
+  \\ Q.SPEC_TAC (`addr32 (ADDR_MODE4_WB am4 x (MAP FST xs))`,`y`)
+  \\ REWRITE_TAC [xR_list_sem_QSORT_INTRO,MEM_MAP_QSORT_INTRO,
+                  ALL_DISTINCT_QSORT_INTRO,LENGTH_QSORT_INTRO]
+  \\ SIMP_TAC std_ss [] \\ Q.SPEC_TAC (`QSORT (\x y. FST x <=+ FST y) xs`,`xs`)
+  \\ Induct \\ REWRITE_TAC [REG_WRITEL_def,MAP,LENGTH,ADDRESS_LIST'_def,ZIP]
+  \\ ASM_SIMP_TAC std_ss [REG_READ_INC_PC,REG_READ_WRITE_NEQ2,MEM,GSYM addr32_SUC]);
+
+val arm_LDM = MAKE_PROG2 raw_LDM ARM_LDM_NOP;
+val arm_LDM = Q.INST [`c`|->`c_flag`,`st`|->`(sN,sZ,sC,Sv)`,`am4`|->`a_mode`] arm_LDM;
+
+val raw_LDM_PC = prove(
+  ``ARM_PROG 
+     (R30 a x * 
+      xR_list (MAP (\x.(FST x,NONE)) xs) * 
+      ms (ADDR_MODE4_ADDR am4 x ((15w,addr32 p)::xs)) 
+         (reg_values ((15w,addr32 p)::xs)) * S st * PASS c st) 
+     [enc (LDM c (ADDR_MODE4_CMD am4) a (reg_bitmap (15w :: MAP FST xs)))] {} SEP_F
+     {(R30 a (ADDR_MODE4_WB am4 x ((15w,addr32 p)::xs)) *
+       xR_list (MAP (\x.(FST x,SOME (SND x))) xs) *
+       ms (ADDR_MODE4_ADDR am4 x ((15w,addr32 p)::xs)) (reg_values ((15w,addr32 p)::xs)) * S st,pcSET p)}``,
+  ARM_PROG_INIT_TAC \\ SIMP_TAC (bool_ss++sep_ss) [pcSET_def] \\ REWRITE_TAC [SEP_F_def]
+  \\ ASM_MOVE_STAR_TAC `a*xs*mm*st*cd*cmd*pc*ud` `pc*a*xs*cmd*mm*st*ud*cd`
+  \\ MOVE_STAR_TAC `a*xs*mm*st*cmd*pc*ud` `pc*a*xs*cmd*mm*st*ud`
+  \\ FULL_SIMP_TAC bool_ss [R30_def,LDM_PRE_EXPANSION,LDM_POST_EXPANSION,
+         LDM_SIMP_LEMMA,ALL_DISTINCT,MEM]
+  \\ `CONDITION_PASSED2 (status s) c` by METIS_TAC []
+  \\ `mem (addr30 (reg 15w s)) s =
+      enc (LDM c (ADDR_MODE4_CMD am4) a (reg_bitmap (15w::MAP FST xs)))` 
+         by METIS_TAC [addr30_addr32]
+  \\ `~(a = 15w)` by METIS_TAC []
+  \\ ASSUME_TAC ((UNDISCH o UNDISCH o UNDISCH o UNDISCH o UNDISCH o UNDISCH o UNDISCH o 
+                  SIMP_RULE std_ss [MAP,ALL_DISTINCT,GSYM AND_IMP_INTRO] o
+                  Q.INST [`p`|->`x`,`Rd`|->`a`,`xs`|->`(15w,addr32 p)::xs`]) ldm)
+  \\ ASM_REWRITE_TAC [] \\ PAT_ASSUM `` NEXT_ARM_MEM s = s'`` (fn th => ALL_TAC)
+  \\ `ALL_DISTINCT (MAP FST ((15w,addr32 p)::xs))` by ASM_SIMP_TAC std_ss [ALL_DISTINCT,MAP]
+  \\ `~MEM a (MAP FST ((15w,addr32 p)::xs))` by ASM_SIMP_TAC std_ss [MEM,MAP]
+  \\ ASM_SIMP_TAC bool_ss [reg_15_LDM_STATE,reg_wb_LDM_STATE,xR_list_sem_LDM_STATE,
+       status_LDM_STATE,mem_LDM_STATE,ms_sem_LDM_STATE,undef_LDM_STATE]
+  \\ STRIP_TAC THEN1 
+    (ONCE_REWRITE_TAC [GSYM xR_list_sem_def]
+     \\ `(15w,SOME (addr32 p))::MAP (\x. (FST x,SOME (SND x))) xs = 
+         MAP (\x. (FST x,SOME (SND x))) ((15w,addr32 p)::xs)` by SIMP_TAC std_ss [MAP]  
+     \\ ASM_SIMP_TAC bool_ss [xR_list_sem_LDM_STATE])
+  \\ REWRITE_TAC [arm2set''_EQ,mem_LDM_STATE,owrt_visible_LDM_STATE]
+  \\ SIMP_TAC (srw_ss()) [IN_INSERT,IN_LIST_TO_SET,LDM_STATE_def,reg_def,state_mode_simp]
+  \\ `LENGTH xs = LENGTH (MAP FST xs)` by METIS_TAC [LENGTH_MAP]
+  \\ `15w::(MAP FST xs) = MAP FST ((15w,addr32 p)::xs)` by SIMP_TAC std_ss [MAP]
+  \\ ASM_SIMP_TAC bool_ss [LEAST_SORT_EQ_QSORT]
+  \\ Q.SPEC_TAC (`ADDR_MODE4_ADDR am4 x (MAP FST ((15w,addr32 p)::xs))`,`ax`)
+  \\ Q.SPEC_TAC (`addr32 (ADDR_MODE4_WB am4 x (MAP FST ((15w,addr32 p)::xs)))`,`y`)
+  \\ `!r a. ~(r = 15w) /\ ~(r = a) /\ ~MEM r (MAP FST xs) =
+         ~(r = 15w) /\ ~(r = a) /\ ~MEM r (MAP FST ((15w,addr32 p)::xs))` by 
+            (SIMP_TAC std_ss [MEM,MAP] \\ METIS_TAC [])
+  \\ `!p. SUC (LENGTH (MAP FST xs)) = LENGTH (MAP FST ((15w,addr32 p)::xs))` by 
+                         (SIMP_TAC std_ss [MEM,MAP,LENGTH] \\ METIS_TAC [])
+  \\ ASM_REWRITE_TAC [] \\ REWRITE_TAC [xR_list_sem_QSORT_INTRO,
+       MEM_MAP_QSORT_INTRO,ALL_DISTINCT_QSORT_INTRO,LENGTH_QSORT_INTRO]
+  \\ SIMP_TAC std_ss [] 
+  \\ Q.SPEC_TAC (`QSORT (\x y. FST x <=+ FST y) ((15w,addr32 p)::xs)`,`xs`)
+  \\ Induct \\ REWRITE_TAC [REG_WRITEL_def,MAP,LENGTH,ADDRESS_LIST'_def,ZIP]
+  \\ ASM_SIMP_TAC std_ss [REG_READ_INC_PC,REG_READ_WRITE_NEQ2,MEM,GSYM addr32_SUC]);
+
+val arm_LDM_PC = MAKE_PROG2 raw_LDM_PC ARM_LDM_NOP;
+val arm_LDM_PC = Q.INST [`c`|->`c_flag`,`st`|->`(sN,sZ,sC,Sv)`,`am4`|->`a_mode`] arm_LDM_PC;
+
+val _ = save_thm("arm_LDM",arm_LDM);
+val _ = save_thm("arm_LDM_PC",arm_LDM_PC);
+
+
+(* STM instruction ------------------------------------------------------------- *)
+
+val STM_STATE_def = Define `
+  STM_STATE am4 x xs a s =
+           <|registers :=
+               INC_PC
+                 (REG_WRITE s.registers (state_mode s) a
+                    (addr32 (ADDR_MODE4_WB am4 x (MAP FST xs))));
+             psrs := s.psrs;
+             memory :=
+               FOLDL
+                 (\mem (rp,rd).
+                    MEM_WRITE_WORD mem rd
+                      (REG_READ
+                         (if HD (LEAST_SORT (MAP FST xs)) = a then
+                            INC_PC s.registers
+                          else
+                            INC_PC
+                              (REG_WRITE s.registers (state_mode s) a
+                                 (addr32
+                                    (ADDR_MODE4_WB am4 x (MAP FST xs)))))
+                         (state_mode s) rp)) s.memory
+                 (ZIP
+                    (LEAST_SORT (MAP FST xs),
+                     ADDR_MODE4_ADDRESSES am4 x (MAP FST xs)));
+             undefined := F|>`;
+
+val stm = simple_clean ARM_STM [``~(Rd = 15w:word4)``]
+val stm = Q.INST [`opt`|->`ADDR_MODE4_CMD am4`] stm
+val stm = Q.INST [`list`|->`reg_bitmap (MAP FST (xs:(word4 # word32) list))`] stm
+val stm = REWRITE_RULE [NOT_ADDR_MODE4_BSN] stm
+val stm = DISCH ``reg Rd s = addr32 p`` stm
+val stm = DISCH ``ALL_DISTINCT (MAP FST (xs:(word4 # word32) list))`` stm
+val stm = SIMP_RULE bool_ss [ADDR_MODE4_FORMAT,FST,SND,ADDR_MODE4_WB_THM] stm
+val stm = REWRITE_RULE [GSYM STM_STATE_def] stm
+
+val status_STM_STATE = prove(
+  ``status (STM_STATE am4 x xs a s) = status s``,
+  SRW_TAC [] [STM_STATE_def,status_def,statusN_def,statusZ_def,statusC_def,statusV_def]);
+
+val undef_STM_STATE = prove(
+  ``(STM_STATE am4 x xs a s).undefined = F``, SRW_TAC [] [STM_STATE_def]);
+
+val owrt_visible_STM_STATE = prove(
+  ``owrt_visible (STM_STATE am4 x xs a s) = owrt_visible s``,
+  SRW_TAC [] [owrt_visible_def,STM_STATE_def,set_status_def,owrt_visible_regs_def,
+              state_mode_simp,REG_OWRT_ALL]);
+
+val reg_15_STM_STATE = prove(
+  ``~(a = 15w) /\ (reg 15w s = addr32 p) ==> 
+    (reg 15w (STM_STATE am4 x xs a s) = addr32 (pcADD 1w p))``,
+  SIMP_TAC (srw_ss()) [STM_STATE_def,reg_def,INC_PC_r15,pcADD_def,
+                       REG_WRITE_r15,GSYM addr32_SUC] \\ METIS_TAC [WORD_ADD_COMM]);
+
+val reg_wb_STM_STATE = prove(
+  ``~(a = 15w) ==> 
+    (reg a (STM_STATE am4 x xs a s) = addr32 (ADDR_MODE4_WB am4 x xs))``,
+  SIMP_TAC (srw_ss()) [STM_STATE_def,reg_def,state_mode_simp,REG_READ_INC_PC,
+                       REG_READ_WRITE,ADDR_MODE4_WB_def,LENGTH_MAP]);
+
+val reg_STM_STATE = prove(
+  ``~(r = 15w) /\ ~(r = a) ==> (reg r (STM_STATE am4 x xs a s) = reg r s)``,
+  SIMP_TAC (srw_ss()) [STM_STATE_def,reg_def,state_mode_simp,REG_READ_INC_PC,
+                       REG_READ_WRITE_NEQ2,LENGTH_MAP]);
+
+val xR_list_sem_STM_STATE = prove(
+  ``xR_list_sem (MAP (\x. (FST x,SOME (SND x))) xs) s /\
+    ~MEM 15w (MAP FST xs) /\ ~MEM a (MAP FST xs) ==>
+    (xR_list_sem (MAP (\x. (FST x,SOME (SND x))) xs) (STM_STATE am4 x xs a s) = 
+     xR_list_sem (MAP (\x. (FST x,SOME (SND x))) xs) s)``,
+  REWRITE_TAC [STM_STATE_def]
+  \\ Q.SPEC_TAC (`FOLDL
+      (\mem (rp,rd). MEM_WRITE_WORD mem rd (REG_READ
+      (if HD (LEAST_SORT (MAP FST xs)) = a then INC_PC s.registers else
+      INC_PC (REG_WRITE s.registers (state_mode s) a
+      (addr32 (ADDR_MODE4_WB am4 x (MAP FST xs))))) (state_mode s) rp)) s.memory
+      (ZIP (LEAST_SORT (MAP FST xs), ADDR_MODE4_ADDRESSES am4 x (MAP FST xs)))`,`fff`)
+  \\ Q.SPEC_TAC (`ADDR_MODE4_WB am4 x (MAP FST xs)`,`wbwb`)
+  \\ Induct_on `xs` \\ SIMP_TAC std_ss [xR_list_sem_def,MAP]
+  \\ Cases \\ Cases_on `q = 15w` \\ ASM_SIMP_TAC std_ss [MEM] 
+  \\ ASM_SIMP_TAC (srw_ss()) [MEM,reg_def,state_mode_simp,
+       REG_READ_INC_PC,REG_READ_WRITE_NEQ2]);
+
+val DISJOINT_SING = prove(
+  ``!p s. DISJOINT {p} s = ~(p IN s)``,
+  SRW_TAC [] [DISJOINT_DEF,EXTENSION,IN_INTER,IN_INSERT,NOT_IN_EMPTY]);
+
+val mem_STM_STATE = prove(
+  ``ALL_DISTINCT (MAP FST xs) /\
+    ~(p IN ms_address_set (ADDR_MODE4_ADDR am4 x xs) (LENGTH xs)) ==>
+    (mem p (STM_STATE am4 x xs a s) = mem p s)``,
+  REWRITE_TAC [STM_STATE_def,ADDR_MODE4_WB_def,LENGTH_MAP]
+  \\ Q.SPEC_TAC (`HD (LEAST_SORT (MAP FST xs)) = a`,`rt`)
+  \\ Q.SPEC_TAC (`(if ADDR_MODE4_wb am4 then ADDR_MODE4_WB' am4 x (LENGTH xs) else x)`,`rt'`)
+  \\ REWRITE_TAC [GSYM ADDR_MODE4_WB_def,ADDR_MODE4_ADDRESSES_def]  
+  \\ `LENGTH xs = LENGTH (MAP FST xs)` by METIS_TAC [LENGTH_MAP] 
+  \\ ASM_REWRITE_TAC [ADDR_MODE4_ADDR_def]
+  \\ REWRITE_TAC [GSYM ADDR_MODE4_ADDR_def]
+  \\ Q.SPEC_TAC (`ADDR_MODE4_ADDR am4 x (MAP FST xs)`,`ax`)
+  \\ SIMP_TAC bool_ss [LEAST_SORT_EQ_QSORT,mem_def]
+  \\ REWRITE_TAC [xR_list_sem_QSORT_INTRO,MEM_MAP_QSORT_INTRO,
+                  ALL_DISTINCT_QSORT_INTRO,LENGTH_QSORT_INTRO]
+  \\ Q.SPEC_TAC (`s.memory`,`mmm`)
+  \\ SIMP_TAC std_ss [] \\ Q.SPEC_TAC (`QSORT (\x y. FST x <=+ FST y) xs`,`xs`)
+  \\ SIMP_TAC (srw_ss()) [] \\ POP_ASSUM (fn th => ALL_TAC)
+  \\ Induct \\ ASM_SIMP_TAC std_ss [LENGTH,ADDRESS_LIST'_def,MAP,ZIP,
+       FOLDL,GSYM addr32_SUC,ALL_DISTINCT,ms_address_set_def,IN_INSERT]
+  \\ SIMP_TAC std_ss [MEM_WRITE_WORD_def,SUBST_def,ADDR30_def,GSYM addr30_def,addr30_addr32]);
+
+val ms_sem_STM_STATE_LEMMA = prove(
+  ``!mmm bx f. 
+      ~MEM (addr32 ax) (ADDRESS_LIST' (addr32 bx) (LENGTH xs)) ==> 
+      (FOLDL
+         (\mem (rp,rd). MEM_WRITE_WORD mem rd (f rp))
+         (MEM_WRITE_WORD mmm (addr32 ax) r)
+         (ZIP (MAP FST xs,ADDRESS_LIST' (addr32 bx) (LENGTH xs))) =
+      MEM_WRITE_WORD
+       (FOLDL
+         (\mem (rp,rd). MEM_WRITE_WORD mem rd (f rp)) mmm
+         (ZIP (MAP FST xs,ADDRESS_LIST' (addr32 bx) (LENGTH xs))))
+     (addr32 ax) r)``,
+  Induct_on `xs` 
+  \\ SIMP_TAC std_ss [MAP,LENGTH,ADDRESS_LIST'_def,ZIP,FOLDL,MEM,GSYM addr32_SUC]
+  \\ Cases \\ REPEAT STRIP_TAC
+  \\ `!x. MEM_WRITE_WORD (MEM_WRITE_WORD mmm (addr32 ax) r) (addr32 bx) x = 
+          MEM_WRITE_WORD (MEM_WRITE_WORD mmm (addr32 bx) x) (addr32 ax) r` by
+        (SRW_TAC [] [MEM_WRITE_WORD_def,SUBST_def,FUN_EQ_THM,ADDR30_def,
+           GSYM addr30_def,addr30_addr32] \\ METIS_TAC [])
+  \\ ASM_REWRITE_TAC [] \\ ASM_SIMP_TAC std_ss []);
+
+val MEM_ADDRESS_LIST' = prove(
+  ``!n a b. MEM (addr32 a) (ADDRESS_LIST' (addr32 b) n) = a IN ms_address_set b n``,
+  Induct \\ ASM_REWRITE_TAC [ADDRESS_LIST'_def,MEM,ms_address_set_def,
+     NOT_IN_EMPTY,IN_INSERT,GSYM addr32_SUC,addr32_11]);
+
+val no_overlap_ADDRESS_LIST' = prove(
+  ``!xs ax. LENGTH xs < 2**30 ==> 
+            ~MEM (addr32 ax) (ADDRESS_LIST' (addr32 (ax+1w)) (LENGTH xs))``,
+  SIMP_TAC bool_ss [MEM_ADDRESS_LIST',IN_ms_address_set]
+  \\ REPEAT STRIP_TAC \\ Cases_on `k < LENGTH xs` \\ ASM_REWRITE_TAC []
+  \\ `n2w k + (ax + 1w) = ax + n2w (k + 1)` by 
+       METIS_TAC [word_add_n2w,WORD_ADD_COMM,WORD_ADD_ASSOC]
+  \\ ONCE_REWRITE_TAC [EQ_SYM_EQ]
+  \\ ASM_REWRITE_TAC [WORD_ADD_RID_UNIQ]  
+  \\ `k + 1 < 2**30` by DECIDE_TAC
+  \\ FULL_SIMP_TAC (std_ss++wordsLib.SIZES_ss) [n2w_11]);
+  
+val ms_sem_STM_STATE = prove(
+  ``LENGTH xs <= 2**30 /\
+    ~MEM a (MAP FST xs) /\ ~MEM 15w (MAP FST xs) /\ ALL_DISTINCT (MAP FST xs) /\ 
+    xR_list_sem (MAP (\x. (FST x,SOME (SND x))) xs) s ==>
+    ms_sem (ADDR_MODE4_ADDR am4 x xs) (reg_values xs) (STM_STATE am4 x xs a s)``,
+  REWRITE_TAC [STM_STATE_def,ADDR_MODE4_WB_def,LENGTH_MAP]
+  \\ Q.SPEC_TAC (`HD (LEAST_SORT (MAP FST xs)) = a`,`rt`)
+  \\ Q.SPEC_TAC (`(if ADDR_MODE4_wb am4 then ADDR_MODE4_WB' am4 x (LENGTH xs) else x)`,`rt'`)
+  \\ REWRITE_TAC [GSYM ADDR_MODE4_WB_def,ADDR_MODE4_ADDRESSES_def]  
+  \\ `LENGTH xs = LENGTH (MAP FST xs)` by METIS_TAC [LENGTH_MAP] 
+  \\ ASM_REWRITE_TAC [ADDR_MODE4_ADDR_def]
+  \\ REWRITE_TAC [GSYM ADDR_MODE4_ADDR_def]
+  \\ Q.SPEC_TAC (`ADDR_MODE4_ADDR am4 x (MAP FST xs)`,`ax`)
+  \\ SIMP_TAC bool_ss [LEAST_SORT_EQ_QSORT,mem_def]
+  \\ REWRITE_TAC [xR_list_sem_QSORT_INTRO,MEM_MAP_QSORT_INTRO,
+                  ALL_DISTINCT_QSORT_INTRO,LENGTH_QSORT_INTRO]
+  \\ Q.SPEC_TAC (`s.memory`,`mmm`)
+  \\ SIMP_TAC std_ss [reg_values_def] 
+  \\ Q.SPEC_TAC (`QSORT (\x y. FST x <=+ FST y) xs`,`xs`)
+  \\ SIMP_TAC (srw_ss()) [] \\ POP_ASSUM (fn th => ALL_TAC)
+  \\ Induct THEN1 REWRITE_TAC [ms_sem_def,MAP]
+  \\ Cases \\ SIMP_TAC std_ss [MAP,HD,MEM,LENGTH,ADDRESS_LIST'_def,ZIP,FOLDL,
+       ALL_DISTINCT,xR_list_sem_def,ms_sem_def,GSYM addr32_SUC] 
+  \\ Cases_on `q = 15w` \\ ASM_REWRITE_TAC []
+  \\ NTAC 5 STRIP_TAC \\ `LENGTH xs <= 1073741824` by DECIDE_TAC
+  \\ `LENGTH xs < 1073741824` by DECIDE_TAC 
+  \\ FULL_SIMP_TAC bool_ss [GSYM (EVAL ``2**30``)] 
+  \\ `~MEM (addr32 ax) (ADDRESS_LIST' (addr32 (ax + 1w)) (LENGTH xs))` 
+        by METIS_TAC [no_overlap_ADDRESS_LIST']
+  \\ ASM_SIMP_TAC bool_ss [ms_sem_STM_STATE_LEMMA]
+  \\ SIMP_TAC (srw_ss()) [mem_def,MEM_WRITE_WORD_def,ADDR30_def,
+         GSYM addr30_def,addr30_addr32,SUBST_def]
+  \\ `REG_READ s.registers (state_mode s) q = r` by METIS_TAC [reg_def]
+  \\ Cases_on `rt` \\ FULL_SIMP_TAC std_ss [REG_READ_INC_PC,REG_READ_WRITE_NEQ2]);
+
+val STM_PRE_EXPANSION = let
+  val xs = `(15w,SOME x1)::(a,SOME x2)::xs`;
+  val ys = `[(b1,xM_seq [y1]);(b3,xM_blank y3)]`;
+  val (st,ud,rt,cd) = (`(T,st)`,`(T,ud)`,`(F,rt)`,`(T,g)`);
+  val th = sep_pred_semantics (xs,ys,st,ud,rt,cd);
+  in th end;
+
+val STM_POST_EXPANSION = LDM_POST_EXPANSION;
+
+val raw_STM = prove(
+  ``ARM_PROG 
+     (R30 a x * 
+      xR_list (MAP (\x.(FST x,SOME (SND x))) xs) * 
+      blank_ms (ADDR_MODE4_ADDR am4 x xs) (LENGTH xs) * S st * PASS c st) 
+     [enc (STM c (ADDR_MODE4_CMD am4) a (reg_bitmap (MAP FST xs)))] {}
+     (R30 a (ADDR_MODE4_WB am4 x xs) *
+      xR_list (MAP (\x.(FST x,SOME (SND x))) xs) *
+      ms (ADDR_MODE4_ADDR am4 x xs) (reg_values xs) * S st) {}``,
+  ARM_PROG_INIT_TAC 
+  \\ ASM_MOVE_STAR_TAC `a*xs*mm*st*cd*cmd*pc*ud` `pc*a*xs*cmd*mm*st*ud*cd`
+  \\ MOVE_STAR_TAC `a*xs*mm*st*cmd*pc*ud` `pc*a*xs*cmd*mm*st*ud`
+  \\ FULL_SIMP_TAC bool_ss [R30_def,STM_PRE_EXPANSION,STM_POST_EXPANSION,DISJOINT_SING,
+         LDM_SIMP_LEMMA,ALL_DISTINCT,MEM,LENGTH_reg_values,ALL_DISJOINT_def,EVERY_DEF]
+  \\ `CONDITION_PASSED2 (status s) c` by METIS_TAC []
+  \\ `mem (addr30 (reg 15w s)) s =
+      enc (STM c (ADDR_MODE4_CMD am4) a (reg_bitmap (MAP FST xs)))` 
+         by METIS_TAC [addr30_addr32]
+  \\ `~(a = 15w)` by METIS_TAC []
+  \\ ASSUME_TAC ((UNDISCH o UNDISCH o UNDISCH o UNDISCH o UNDISCH o UNDISCH o 
+                  Q.INST [`p`|->`x`,`Rd`|->`a`]) stm)
+  \\ ASM_REWRITE_TAC [] \\ PAT_ASSUM `` NEXT_ARM_MEM s = s'`` (fn th => ALL_TAC)
+  \\ ASM_SIMP_TAC bool_ss [status_STM_STATE,undef_STM_STATE,reg_15_STM_STATE,
+       reg_wb_STM_STATE,xR_list_sem_STM_STATE,mem_STM_STATE,ms_sem_STM_STATE]
+  \\ ASM_SIMP_TAC bool_ss [arm2set''_EQ,owrt_visible_STM_STATE,IN_INSERT,
+       reg_STM_STATE,mem_STM_STATE]);
+
+val arm_STM = MAKE_PROG2 raw_STM ARM_STM_NOP;
+val arm_STM = Q.INST [`c`|->`c_flag`,`st`|->`(sN,sZ,sC,Sv)`,`am4`|->`a_mode`] arm_STM;
+
+val _ = save_thm("arm_STM",arm_STM);
+
 
 val _ = export_theory();
 
